# baseURI: http://anzsoil.org/def/au/asls/land-surface
# imports: http://anzsoil.org/def/au/asls/substrate
# imports: http://purl.org/dc/elements/1.1/
# imports: http://purl.org/linked-data/registry
# imports: http://purl.org/linked-data/registry-ui#
# imports: http://www.w3.org/ns/sosa/

@prefix asls: <http://anzsoil.org/def/au/asls/> .
@prefix dc: <http://purl.org/dc/elements/1.1/> .
@prefix dcterms: <http://purl.org/dc/terms/> .
@prefix ls: <http://anzsoil.org/def/au/asls/land-surface/> .
@prefix owl: <http://www.w3.org/2002/07/owl#> .
@prefix rdf: <http://www.w3.org/1999/02/22-rdf-syntax-ns#> .
@prefix rdfs: <http://www.w3.org/2000/01/rdf-schema#> .
@prefix reg: <http://purl.org/linked-data/registry#> .
@prefix skos: <http://www.w3.org/2004/02/skos/core#> .
@prefix sosa: <http://www.w3.org/ns/sosa/> .
@prefix sp: <http://anzsoil.org/def/au/asls/soil-profile/> .
@prefix subst: <http://anzsoil.org/def/au/asls/substrate/> .
@prefix ui: <http://purl.org/linked-data/registry-ui#> .
@prefix xsd: <http://www.w3.org/2001/XMLSchema#> .

 <aggradation>
  a skos:Collection ;
  a sosa:ObservableProperty ;
  dcterms:description "This refers to the presence of material deposited on a pre-existing surface as a result of wind and/or water erosion."@en ;
  dcterms:identifier "http://anzsoil.org/def/au/asls/land-surface/aggradation"^^xsd:anyURI ;
  ui:topMemberOf <> ;
  rdfs:label "Aggradation"@en ;
  skos:definition "This refers to the presence of material deposited on a pre-existing surface as a result of wind and/or water erosion."@en ;
  skos:member  <aggradation-0> ;
  skos:member  <aggradation-1> ;
  skos:member  <aggradation-X> ;
  skos:prefLabel "Aggradation"@en ;
.
 <aggradation-0>
  a skos:Concept ;
  dcterms:description "No aggradation."@en ;
  dcterms:identifier "http://anzsoil.org/def/au/asls/land-surface/aggradation-0"^^xsd:anyURI ;
  ui:isMemberOf  <aggradation> ;
  rdfs:label "No aggradation"@en ;
  skos:definition "No aggradation."@en ;
  skos:inScheme <> ;
  skos:notation "0" ;
  skos:prefLabel "No aggradation"@en ;
  skos:topConceptOf <> ;
.
 <aggradation-1>
  a skos:Concept ;
  dcterms:description "Aggradation present."@en ;
  dcterms:identifier "http://anzsoil.org/def/au/asls/land-surface/aggradation-1"^^xsd:anyURI ;
  ui:isMemberOf  <aggradation> ;
  rdfs:label "Present"@en ;
  skos:definition "Aggradation present."@en ;
  skos:inScheme <> ;
  skos:notation "1" ;
  skos:prefLabel "Present"@en ;
  skos:topConceptOf <> ;
.
 <aggradation-X>
  a skos:Concept ;
  dcterms:description "Aggradation not apparent."@en ;
  dcterms:identifier "http://anzsoil.org/def/au/asls/land-surface/aggradation-X"^^xsd:anyURI ;
  ui:isMemberOf  <aggradation> ;
  rdfs:label "Not apparent"@en ;
  skos:definition "Aggradation not apparent."@en ;
  skos:inScheme <> ;
  skos:notation "X" ;
  skos:prefLabel "Not apparent"@en ;
  skos:topConceptOf <> ;
.
 <aspect>
  a skos:Concept ;
  a sosa:ObservableProperty ;
  dcterms:description "Give as compass bearing to nearest 10 degrees. On level lands (less than 1% slope), aspect need not be recorded."@en ;
  dcterms:identifier "http://anzsoil.org/def/au/asls/land-surface/aspect"^^xsd:anyURI ;
  ui:topMemberOf <> ;
  rdfs:label "Aspect"@en ;
  skos:definition "Give as compass bearing to nearest 10 degrees. On level lands (less than 1% slope), aspect need not be recorded."@en ;
  skos:inScheme <> ;
  skos:prefLabel "Aspect"@en ;
  skos:topConceptOf <> ;
.
 <biotic-microrelief>
  a skos:Collection ;
  dcterms:description "This relief is caused by biotic agents, for example termite mounds, rabbit warrens, wombat burrows, pig wallows, man-made terraces, stump holes, vegetation mounds. No subdivision of any of the types of biotic microrelief according to the specific agent or component of relief is given here. For example, vegetation mounds are mounds of soil material found at the base of plants such as Dillon bush (Nitraria billardieri) or spinifex (Triodia species). Users may subdivide types of biotic microrelief where considered necessary, such as specifying the particular species of vegetation involved in the case of vegetation mounds. For example, termite mounds would be coded TM."@en ;
  dcterms:identifier "http://anzsoil.org/def/au/asls/land-surface/biotic-microrelief"^^xsd:anyURI ;
  ui:isMemberOf  <microrelief> ;
  rdfs:label "Biotic microreliefs"@en ;
  skos:definition "This relief is caused by biotic agents, for example termite mounds, rabbit warrens, wombat burrows, pig wallows, man-made terraces, stump holes, vegetation mounds. No subdivision of any of the types of biotic microrelief according to the specific agent or component of relief is given here. For example, vegetation mounds are mounds of soil material found at the base of plants such as Dillon bush (Nitraria billardieri) or spinifex (Triodia species). Users may subdivide types of biotic microrelief where considered necessary, such as specifying the particular species of vegetation involved in the case of vegetation mounds. For example, termite mounds would be coded TM."@en ;
  skos:member  <biotic-microrelief-agents> ;
  skos:member  <biotic-microrelief-components> ;
  skos:prefLabel "Biotic microrelief"@en ;
.
 <biotic-microrelief-agent-A>
  a skos:Concept ;
  dcterms:description "Ant."@en ;
  dcterms:identifier "http://anzsoil.org/def/au/asls/land-surface/biotic-microrelief-agent-A"^^xsd:anyURI ;
  ui:isMemberOf  <biotic-microrelief-agents> ;
  rdfs:label "Ant"@en ;
  skos:definition "Ant."@en ;
  skos:inScheme <> ;
  skos:notation "A" ;
  skos:prefLabel "Ant"@en ;
  skos:topConceptOf <> ;
.
 <biotic-microrelief-agent-B>
  a skos:Concept ;
  dcterms:description "Bird."@en ;
  dcterms:identifier "http://anzsoil.org/def/au/asls/land-surface/biotic-microrelief-agent-B"^^xsd:anyURI ;
  ui:isMemberOf  <biotic-microrelief-agents> ;
  rdfs:label "Bird"@en ;
  skos:definition "Bird."@en ;
  skos:inScheme <> ;
  skos:notation "B" ;
  skos:prefLabel "Bird"@en ;
  skos:topConceptOf <> ;
.
 <biotic-microrelief-agent-M>
  a skos:Concept ;
  dcterms:description "Human."@en ;
  dcterms:identifier "http://anzsoil.org/def/au/asls/land-surface/biotic-microrelief-agent-M"^^xsd:anyURI ;
  ui:isMemberOf  <biotic-microrelief-agents> ;
  rdfs:label "Human"@en ;
  skos:definition "Human."@en ;
  skos:inScheme <> ;
  skos:notation "M" ;
  skos:prefLabel "Human"@en ;
  skos:topConceptOf <> ;
.
 <biotic-microrelief-agent-N>
  a skos:Concept ;
  dcterms:description "Animal."@en ;
  dcterms:identifier "http://anzsoil.org/def/au/asls/land-surface/biotic-microrelief-agent-N"^^xsd:anyURI ;
  ui:isMemberOf  <biotic-microrelief-agents> ;
  rdfs:label "Animal"@en ;
  skos:definition "Animal."@en ;
  skos:inScheme <> ;
  skos:notation "N" ;
  skos:prefLabel "Animal"@en ;
  skos:topConceptOf <> ;
.
 <biotic-microrelief-agent-O>
  a skos:Concept ;
  dcterms:description "Other."@en ;
  dcterms:identifier "http://anzsoil.org/def/au/asls/land-surface/biotic-microrelief-agent-O"^^xsd:anyURI ;
  ui:isMemberOf  <biotic-microrelief-agents> ;
  rdfs:label "Other"@en ;
  skos:definition "Other."@en ;
  skos:inScheme <> ;
  skos:notation "O" ;
  skos:prefLabel "Other"@en ;
  skos:topConceptOf <> ;
.
 <biotic-microrelief-agent-T>
  a skos:Concept ;
  dcterms:description "Termite."@en ;
  dcterms:identifier "http://anzsoil.org/def/au/asls/land-surface/biotic-microrelief-agent-T"^^xsd:anyURI ;
  ui:isMemberOf  <biotic-microrelief-agents> ;
  rdfs:label "Termite"@en ;
  skos:definition "Termite."@en ;
  skos:inScheme <> ;
  skos:notation "T" ;
  skos:prefLabel "Termite"@en ;
  skos:topConceptOf <> ;
.
 <biotic-microrelief-agent-V>
  a skos:Concept ;
  dcterms:description "Vegetation."@en ;
  dcterms:identifier "http://anzsoil.org/def/au/asls/land-surface/biotic-microrelief-agent-V"^^xsd:anyURI ;
  ui:isMemberOf  <biotic-microrelief-agents> ;
  rdfs:label "Vegetation"@en ;
  skos:definition "Vegetation."@en ;
  skos:inScheme <> ;
  skos:notation "V" ;
  skos:prefLabel "Vegetation"@en ;
  skos:topConceptOf <> ;
.
 <biotic-microrelief-agents>
  a skos:Collection ;
  a sosa:ObservableProperty ;
  dcterms:description "The biotic agents causing the relief. "@en ;
  dcterms:identifier "http://anzsoil.org/def/au/asls/land-surface/biotic-microrelief-agents"^^xsd:anyURI ;
  ui:isMemberOf  <biotic-microrelief> ;
  rdfs:label "Biotic microrelief agents"@en ;
  skos:definition "The biotic agents causing the relief."@en ;
  skos:member  <biotic-microrelief-agent-A> ;
  skos:member  <biotic-microrelief-agent-B> ;
  skos:member  <biotic-microrelief-agent-M> ;
  skos:member  <biotic-microrelief-agent-N> ;
  skos:member  <biotic-microrelief-agent-O> ;
  skos:member  <biotic-microrelief-agent-T> ;
  skos:member  <biotic-microrelief-agent-V> ;
  skos:prefLabel "Biotic microrelief agents"@en ;
.
 <biotic-microrelief-component-D>
  a skos:Concept ;
  dcterms:description "Depression."@en ;
  dcterms:identifier "http://anzsoil.org/def/au/asls/land-surface/biotic-microrelief-component-D"^^xsd:anyURI ;
  ui:isMemberOf  <biotic-microrelief-components> ;
  rdfs:label "Depression"@en ;
  skos:definition "Depression."@en ;
  skos:inScheme <> ;
  skos:notation "D" ;
  skos:prefLabel "Depression"@en ;
  skos:topConceptOf <> ;
.
 <biotic-microrelief-component-E>
  a skos:Concept ;
  dcterms:description "Elongate mound."@en ;
  dcterms:identifier "http://anzsoil.org/def/au/asls/land-surface/biotic-microrelief-component-E"^^xsd:anyURI ;
  ui:isMemberOf  <biotic-microrelief-components> ;
  rdfs:label "Elongate mound"@en ;
  skos:definition "Elongate mound."@en ;
  skos:inScheme <> ;
  skos:notation "E" ;
  skos:prefLabel "Elongate mound"@en ;
  skos:topConceptOf <> ;
.
 <biotic-microrelief-component-H>
  a skos:Concept ;
  dcterms:description "Hole."@en ;
  dcterms:identifier "http://anzsoil.org/def/au/asls/land-surface/biotic-microrelief-component-H"^^xsd:anyURI ;
  ui:isMemberOf  <biotic-microrelief-components> ;
  rdfs:label "Hole"@en ;
  skos:definition "Hole."@en ;
  skos:inScheme <> ;
  skos:notation "H" ;
  skos:prefLabel "Hole"@en ;
  skos:topConceptOf <> ;
.
 <biotic-microrelief-component-L>
  a skos:Concept ;
  dcterms:description "Elongate depression."@en ;
  dcterms:identifier "http://anzsoil.org/def/au/asls/land-surface/biotic-microrelief-component-L"^^xsd:anyURI ;
  ui:isMemberOf  <biotic-microrelief-components> ;
  rdfs:label "Elongate depression"@en ;
  skos:definition "Elongate depression."@en ;
  skos:inScheme <> ;
  skos:notation "L" ;
  skos:prefLabel "Elongate depression"@en ;
  skos:topConceptOf <> ;
.
 <biotic-microrelief-component-M>
  a skos:Concept ;
  dcterms:description "Mound."@en ;
  dcterms:identifier "http://anzsoil.org/def/au/asls/land-surface/biotic-microrelief-component-M"^^xsd:anyURI ;
  ui:isMemberOf  <biotic-microrelief-components> ;
  rdfs:label "Mound"@en ;
  skos:definition "Mound."@en ;
  skos:inScheme <> ;
  skos:notation "M" ;
  skos:prefLabel "Mound"@en ;
  skos:topConceptOf <> ;
.
 <biotic-microrelief-component-O>
  a skos:Concept ;
  dcterms:description "Other."@en ;
  dcterms:identifier "http://anzsoil.org/def/au/asls/land-surface/biotic-microrelief-component-O"^^xsd:anyURI ;
  ui:isMemberOf  <biotic-microrelief-components> ;
  rdfs:label "Other."@en ;
  skos:definition "Other.."@en ;
  skos:inScheme <> ;
  skos:notation "O" ;
  skos:prefLabel "Other."@en ;
  skos:topConceptOf <> ;
.
 <biotic-microrelief-component-T>
  a skos:Concept ;
  dcterms:description "Terrace."@en ;
  dcterms:identifier "http://anzsoil.org/def/au/asls/land-surface/biotic-microrelief-component-T"^^xsd:anyURI ;
  ui:isMemberOf  <biotic-microrelief-components> ;
  rdfs:label "Terrace"@en ;
  skos:definition "Terrace."@en ;
  skos:inScheme <> ;
  skos:notation "T" ;
  skos:prefLabel "Terrace"@en ;
  skos:topConceptOf <> ;
.
 <biotic-microrelief-components>
  a skos:Collection ;
  a sosa:ObservableProperty ;
  dcterms:description "The component of the biotic relief."@en ;
  dcterms:identifier "http://anzsoil.org/def/au/asls/land-surface/biotic-microrelief-components"^^xsd:anyURI ;
  ui:isMemberOf  <biotic-microrelief> ;
  rdfs:label "Component of biotic relief"@en ;
  skos:definition "The component of the biotic relief."@en ;
  skos:member  <biotic-microrelief-component-D> ;
  skos:member  <biotic-microrelief-component-E> ;
  skos:member  <biotic-microrelief-component-H> ;
  skos:member  <biotic-microrelief-component-L> ;
  skos:member  <biotic-microrelief-component-M> ;
  skos:member  <biotic-microrelief-component-O> ;
  skos:member  <biotic-microrelief-component-T> ;
  skos:prefLabel "Component of biotic relief"@en ;
.
 <coarse-fragments>
  a skos:Collection ;
  dcterms:description """Coarse fragments are particles coarser than 2 mm. They include unattached rock fragments and other fragments such as charcoal and shells. Coarse fragments are distinguished from segregations of pedogenic origin in that they are not, or not considered to be, of pedogenic origin.  
Both coarse fragments and segregations of pedogenic origin can occur on the surface. Where segregations of pedogenic origin occur on the surface, they should be described as per soil-profile."""@en ;
  dcterms:identifier "http://anzsoil.org/def/au/asls/land-surface/coarse-fragments"^^xsd:anyURI ;
  ui:topMemberOf <> ;
  rdfs:label "Coarse fragments"@en ;
  skos:definition """Coarse fragments are particles coarser than 2 mm. They include unattached rock fragments and other fragments such as charcoal and shells. Coarse fragments are distinguished from segregations of pedogenic origin in that they are not, or not considered to be, of pedogenic origin.  
Both coarse fragments and segregations of pedogenic origin can occur on the surface. Where segregations of pedogenic origin occur on the surface, they should be described as per soil-profile."""@en ;
  skos:member  <coarse-fragments-abundance> ;
  skos:member  <coarse-fragments-lithology> ;
  skos:member  <coarse-fragments-shape> ;
  skos:member  <coarse-fragments-size> ;
  skos:member  <coarse-fragments-strength> ;
  skos:prefLabel "Coarse fragments"@en ;
.
 <coarse-fragments-abundance>
  a skos:Collection ;
  a sosa:ObservableProperty ;
  dcterms:description "<p><img src=\"http://anzsoil.org/resources/yellowbook/Figure11.png\" /></p>"^^rdf:HTML ;
  dcterms:identifier "http://anzsoil.org/def/au/asls/land-surface/coarse-fragments-abundance"^^xsd:anyURI ;
  ui:isMemberOf  <coarse-fragments> ;
  rdfs:comment "The percentage is estimated by eye using the charts in the yellow book for comparison. N_CF_ABUN"@en ;
  rdfs:label "Abundance of coarse fragments"@en ;
  skos:definition "The percentage of coarse fragments."@en ;
  skos:member  <coarse-fragments-abundance-0> ;
  skos:member  <coarse-fragments-abundance-1> ;
  skos:member  <coarse-fragments-abundance-2> ;
  skos:member  <coarse-fragments-abundance-3> ;
  skos:member  <coarse-fragments-abundance-4> ;
  skos:member  <coarse-fragments-abundance-5> ;
  skos:member  <coarse-fragments-abundance-6> ;
  skos:prefLabel "Abundance of coarse fragments"@en ;
.
 <coarse-fragments-abundance-0>
  a skos:Concept ;
  dcterms:description "0%"@en ;
  dcterms:identifier "http://anzsoil.org/def/au/asls/land-surface/coarse-fragments-abundance-0"^^xsd:anyURI ;
  ui:isMemberOf  <coarse-fragments-abundance> ;
  rdfs:comment "The percentage is estimated by eye using the charts in the yellow book for comparison. N_CF_ABUN"@en ;
  rdfs:label "No coarse fragments"@en ;
  skos:definition "0%"@en ;
  skos:inScheme <> ;
  skos:notation "0" ;
  skos:prefLabel "No coarse fragments"@en ;
  skos:topConceptOf <> ;
.
 <coarse-fragments-abundance-1>
  a skos:Concept ;
  dcterms:description "<2%"@en ;
  dcterms:identifier "http://anzsoil.org/def/au/asls/land-surface/coarse-fragments-abundance-1"^^xsd:anyURI ;
  ui:isMemberOf  <coarse-fragments-abundance> ;
  rdfs:comment "The percentage is estimated by eye using the charts in the yellow book for comparison. N_CF_ABUN"@en ;
  rdfs:label "Very slightly or very few, for example very slightly fine gravelly; very few small pebbles"@en ;
  skos:definition "<2%"@en ;
  skos:inScheme <> ;
  skos:notation "1" ;
  skos:prefLabel "Very slightly or very few, for example very slightly fine gravelly; very few small pebbles"@en ;
  skos:topConceptOf <> ;
.
 <coarse-fragments-abundance-2>
  a skos:Concept ;
  dcterms:description "2-10%"@en ;
  dcterms:identifier "http://anzsoil.org/def/au/asls/land-surface/coarse-fragments-abundance-2"^^xsd:anyURI ;
  ui:isMemberOf  <coarse-fragments-abundance> ;
  rdfs:comment "The percentage is estimated by eye using the charts in the yellow book for comparison. N_CF_ABUN"@en ;
  rdfs:label "Slightly or few, for example slightly stony; few stones"@en ;
  skos:definition "2-10%"@en ;
  skos:inScheme <> ;
  skos:notation "2" ;
  skos:prefLabel "Slightly or few, for example slightly stony; few stones"@en ;
  skos:topConceptOf <> ;
.
 <coarse-fragments-abundance-3>
  a skos:Concept ;
  dcterms:description "10-20%"@en ;
  dcterms:identifier "http://anzsoil.org/def/au/asls/land-surface/coarse-fragments-abundance-3"^^xsd:anyURI ;
  ui:isMemberOf  <coarse-fragments-abundance> ;
  rdfs:comment "The percentage is estimated by eye using the charts in the yellow book for comparison: for example medium gravelly; stony, common medium pebbles; common stones. N_CF_ABUN"@en ;
  rdfs:label "No qualifier or common, for example medium gravelly; stony, common medium pebbles; common stones"@en ;
  skos:definition "10-20%"@en ;
  skos:inScheme <> ;
  skos:notation "3" ;
  skos:prefLabel "No qualifier or common, for example medium gravelly; stony, common medium pebbles; common stones"@en ;
  skos:topConceptOf <> ;
.
 <coarse-fragments-abundance-4>
  a skos:Concept ;
  dcterms:description "20-50%"@en ;
  dcterms:identifier "http://anzsoil.org/def/au/asls/land-surface/coarse-fragments-abundance-4"^^xsd:anyURI ;
  ui:isMemberOf  <coarse-fragments-abundance> ;
  rdfs:comment "The percentage is estimated by eye using the charts in the yellow book for comparison. N_CF_ABUN"@en ;
  rdfs:label "Moderately or many"@en ;
  skos:definition "20-50%"@en ;
  skos:inScheme <> ;
  skos:notation "4" ;
  skos:prefLabel "Moderately or many"@en ;
  skos:topConceptOf <> ;
.
 <coarse-fragments-abundance-5>
  a skos:Concept ;
  dcterms:description "50-90%"@en ;
  dcterms:identifier "http://anzsoil.org/def/au/asls/land-surface/coarse-fragments-abundance-5"^^xsd:anyURI ;
  ui:isMemberOf  <coarse-fragments-abundance> ;
  rdfs:comment "The percentage is estimated by eye using the charts in the yellow book for comparison. N_CF_ABUN"@en ;
  rdfs:label "Very or abundant"@en ;
  skos:definition "50-90%"@en ;
  skos:inScheme <> ;
  skos:notation "5" ;
  skos:prefLabel "Very or abundant"@en ;
  skos:topConceptOf <> ;
.
 <coarse-fragments-abundance-6>
  a skos:Concept ;
  dcterms:description ">90%"@en ;
  dcterms:identifier "http://anzsoil.org/def/au/asls/land-surface/coarse-fragments-abundance-6"^^xsd:anyURI ;
  ui:isMemberOf  <coarse-fragments-abundance> ;
  rdfs:comment "The percentage is estimated by eye using the charts in the yellow book for comparison. N_CF_ABUN"@en ;
  rdfs:label "Extremely or very abundant"@en ;
  skos:definition ">90%"@en ;
  skos:inScheme <> ;
  skos:notation "6" ;
  skos:prefLabel "Extremely or very abundant"@en ;
  skos:topConceptOf <> ;
.
 <coarse-fragments-lithology>
  a skos:Collection ;
  a sosa:ObservableProperty ;
  dcterms:description "The lithology of the coarse fragments is usually identified as coming from the substrate or from rock outcrop. Where the lithology of the coarse fragments is different from that of the substrate material and/or rock outcrop, describe it as for lithology of substrate material only where the rock type is definitely known or is confidently presumed. Some coarse fragments are commonly encountered that are not directly related to the substrate material.   "@en ;
  dcterms:identifier "http://anzsoil.org/def/au/asls/land-surface/coarse-fragments-lithology"^^xsd:anyURI ;
  ui:isMemberOf  <coarse-fragments> ;
  rdfs:comment "C_LITHOLOGY" ;
  rdfs:label "Lithology of coarse fragments"@en ;
  skos:definition "The lithology of the coarse fragments is usually identified as coming from the substrate or from rock outcrop. Where the lithology of the coarse fragments is different from that of the substrate material and/or rock outcrop, describe it as for lithology of substrate material only where the rock type is definitely known or is confidently presumed. Some coarse fragments are commonly encountered that are not directly related to the substrate material.    "@en ;
  skos:member  <lithology-CC> ;
  skos:member  <lithology-IS> ;
  skos:member  <lithology-OT> ;
  skos:member  <lithology-OW> ;
  skos:member  <lithology-PU> ;
  skos:member  <lithology-SS> ;
  skos:member  <../substrate/lithology-AC> ;
  skos:member  <../substrate/lithology-AD> ;
  skos:member  <../substrate/lithology-AF> ;
  skos:member  <../substrate/lithology-AG> ;
  skos:member  <../substrate/lithology-AH> ;
  skos:member  <../substrate/lithology-AM> ;
  skos:member  <../substrate/lithology-AN> ;
  skos:member  <../substrate/lithology-AP> ;
  skos:member  <../substrate/lithology-AR> ;
  skos:member  <../substrate/lithology-AS> ;
  skos:member  <../substrate/lithology-BA> ;
  skos:member  <../substrate/lithology-BB> ;
  skos:member  <../substrate/lithology-BR> ;
  skos:member  <../substrate/lithology-C> ;
  skos:member  <../substrate/lithology-CG> ;
  skos:member  <../substrate/lithology-CH> ;
  skos:member  <../substrate/lithology-CO> ;
  skos:member  <../substrate/lithology-CU> ;
  skos:member  <../substrate/lithology-DI> ;
  skos:member  <../substrate/lithology-DM> ;
  skos:member  <../substrate/lithology-DR> ;
  skos:member  <../substrate/lithology-FC> ;
  skos:member  <../substrate/lithology-GA> ;
  skos:member  <../substrate/lithology-GD> ;
  skos:member  <../substrate/lithology-GE> ;
  skos:member  <../substrate/lithology-GN> ;
  skos:member  <../substrate/lithology-GR> ;
  skos:member  <../substrate/lithology-GS> ;
  skos:member  <../substrate/lithology-GV> ;
  skos:member  <../substrate/lithology-GW> ;
  skos:member  <../substrate/lithology-GY> ;
  skos:member  <../substrate/lithology-HA> ;
  skos:member  <../substrate/lithology-HO> ;
  skos:member  <../substrate/lithology-IG> ;
  skos:member  <../substrate/lithology-JA> ;
  skos:member  <../substrate/lithology-KA> ;
  skos:member  <../substrate/lithology-KC> ;
  skos:member  <../substrate/lithology-KL> ;
  skos:member  <../substrate/lithology-KM> ;
  skos:member  <../substrate/lithology-KR> ;
  skos:member  <../substrate/lithology-KS> ;
  skos:member  <../substrate/lithology-LC> ;
  skos:member  <../substrate/lithology-LI> ;
  skos:member  <../substrate/lithology-M> ;
  skos:member  <../substrate/lithology-MB> ;
  skos:member  <../substrate/lithology-MD> ;
  skos:member  <../substrate/lithology-ME> ;
  skos:member  <../substrate/lithology-MG> ;
  skos:member  <../substrate/lithology-MI> ;
  skos:member  <../substrate/lithology-ML> ;
  skos:member  <../substrate/lithology-MS> ;
  skos:member  <../substrate/lithology-MU> ;
  skos:member  <../substrate/lithology-MY> ;
  skos:member  <../substrate/lithology-PC> ;
  skos:member  <../substrate/lithology-PE> ;
  skos:member  <../substrate/lithology-PG> ;
  skos:member  <../substrate/lithology-PH> ;
  skos:member  <../substrate/lithology-PL> ;
  skos:member  <../substrate/lithology-PO> ;
  skos:member  <../substrate/lithology-PY> ;
  skos:member  <../substrate/lithology-QP> ;
  skos:member  <../substrate/lithology-QS> ;
  skos:member  <../substrate/lithology-QU> ;
  skos:member  <../substrate/lithology-QZ> ;
  skos:member  <../substrate/lithology-R> ;
  skos:member  <../substrate/lithology-RB> ;
  skos:member  <../substrate/lithology-RH> ;
  skos:member  <../substrate/lithology-S> ;
  skos:member  <../substrate/lithology-SA> ;
  skos:member  <../substrate/lithology-SD> ;
  skos:member  <../substrate/lithology-SH> ;
  skos:member  <../substrate/lithology-SK> ;
  skos:member  <../substrate/lithology-SL> ;
  skos:member  <../substrate/lithology-SR> ;
  skos:member  <../substrate/lithology-ST> ;
  skos:member  <../substrate/lithology-SY> ;
  skos:member  <../substrate/lithology-TR> ;
  skos:member  <../substrate/lithology-TU> ;
  skos:member  <../substrate/lithology-UC> ;
  skos:member  <../substrate/lithology-VB> ;
  skos:member  <../substrate/lithology-VG> ;
  skos:member  <../substrate/lithology-Z> ;
  skos:member  <../substrate/lithology-ZS> ;
  skos:prefLabel "Lithology of coarse fragments"@en ;
.
 <coarse-fragments-shape>
  a skos:Collection ;
  a sosa:ObservableProperty ;
  dcterms:description "<p><img src=\"http://anzsoil.org/resources/yellowbook/Figure12.png\" /></p>"^^rdf:HTML ;
  dcterms:identifier "http://anzsoil.org/def/au/asls/land-surface/coarse-fragments-shape"^^xsd:anyURI ;
  ui:isMemberOf  <coarse-fragments> ;
  rdfs:comment "C_CF_SHAPE" ;
  rdfs:label "Shape of coarse fragments"@en ;
  skos:definition "The shape of coarse fragments is determined by referencing the chart that captures the roundness and sphericity. (Figure 12)"@en ;
  skos:member  <coarse-fragments-shape-A> ;
  skos:member  <coarse-fragments-shape-AP> ;
  skos:member  <coarse-fragments-shape-AT> ;
  skos:member  <coarse-fragments-shape-R> ;
  skos:member  <coarse-fragments-shape-RP> ;
  skos:member  <coarse-fragments-shape-RT> ;
  skos:member  <coarse-fragments-shape-S> ;
  skos:member  <coarse-fragments-shape-SP> ;
  skos:member  <coarse-fragments-shape-ST> ;
  skos:member  <coarse-fragments-shape-U> ;
  skos:member  <coarse-fragments-shape-UP> ;
  skos:member  <coarse-fragments-shape-UT> ;
  skos:prefLabel "Shape of coarse fragments"@en ;
.
 <coarse-fragments-shape-A>
  a skos:Concept ;
  dcterms:description "Angular shape as determined from visual guide"@en ;
  dcterms:identifier "http://anzsoil.org/def/au/asls/land-surface/coarse-fragments-shape-A"^^xsd:anyURI ;
  ui:isMemberOf  <coarse-fragments-shape> ;
  rdfs:comment "C_CF_SHAPE" ;
  rdfs:label "Angular"@en ;
  skos:definition "Angular shape as determined from visual guide"@en ;
  skos:inScheme <> ;
  skos:notation "A" ;
  skos:prefLabel "Angular"@en ;
  skos:topConceptOf <> ;
.
 <coarse-fragments-shape-AP>
  a skos:Concept ;
  dcterms:description "Angular shape as determined from visual guide"@en ;
  dcterms:identifier "http://anzsoil.org/def/au/asls/land-surface/coarse-fragments-shape-AP"^^xsd:anyURI ;
  ui:isMemberOf  <coarse-fragments-shape> ;
  rdfs:comment "C_CF_SHAPE" ;
  rdfs:label "Angular platy"@en ;
  skos:definition "Angular platy shape as determined from visual guide"@en ;
  skos:inScheme <> ;
  skos:notation "AP" ;
  skos:prefLabel "Angular platy"@en ;
  skos:topConceptOf <> ;
.
 <coarse-fragments-shape-AT>
  a skos:Concept ;
  dcterms:description "Angular tabular shape as determined from visual guide"@en ;
  dcterms:identifier "http://anzsoil.org/def/au/asls/land-surface/coarse-fragments-shape-AT"^^xsd:anyURI ;
  ui:isMemberOf  <coarse-fragments-shape> ;
  rdfs:comment "C_CF_SHAPE" ;
  rdfs:label "Angular tabular"@en ;
  skos:definition "Angular tabular shape as determined from visual guide"@en ;
  skos:inScheme <> ;
  skos:notation "AT" ;
  skos:prefLabel "Angular tabular"@en ;
  skos:topConceptOf <> ;
.
 <coarse-fragments-shape-R>
  a skos:Concept ;
  dcterms:description "Rounded shape as determined from visual guide"@en ;
  dcterms:identifier "http://anzsoil.org/def/au/asls/land-surface/coarse-fragments-shape-R"^^xsd:anyURI ;
  ui:isMemberOf  <coarse-fragments-shape> ;
  rdfs:comment "C_CF_SHAPE" ;
  rdfs:label "Rounded"@en ;
  skos:definition "Rounded shape as determined from visual guide"@en ;
  skos:inScheme <> ;
  skos:notation "R" ;
  skos:prefLabel "Rounded"@en ;
  skos:topConceptOf <> ;
.
 <coarse-fragments-shape-RP>
  a skos:Concept ;
  dcterms:description "Rounded platy shape as determined from visual guide"@en ;
  dcterms:identifier "http://anzsoil.org/def/au/asls/land-surface/coarse-fragments-shape-RP"^^xsd:anyURI ;
  ui:isMemberOf  <coarse-fragments-shape> ;
  rdfs:comment "C_CF_SHAPE" ;
  rdfs:label "Rounded platy"@en ;
  skos:definition "Rounded platy shape as determined from visual guide"@en ;
  skos:inScheme <> ;
  skos:notation "RP" ;
  skos:prefLabel "Rounded platy"@en ;
  skos:topConceptOf <> ;
.
 <coarse-fragments-shape-RT>
  a skos:Concept ;
  dcterms:description "Rounded tabular shape as determined from visual guide"@en ;
  dcterms:identifier "http://anzsoil.org/def/au/asls/land-surface/coarse-fragments-shape-RT"^^xsd:anyURI ;
  ui:isMemberOf  <coarse-fragments-shape> ;
  rdfs:comment "C_CF_SHAPE" ;
  rdfs:label "Rounded tabular"@en ;
  skos:definition "Rounded tabular shape as determined from visual guide"@en ;
  skos:inScheme <> ;
  skos:notation "RT" ;
  skos:prefLabel "Rounded tabular"@en ;
  skos:topConceptOf <> ;
.
 <coarse-fragments-shape-S>
  a skos:Concept ;
  dcterms:description "Subangular shape as determined from visual guide"@en ;
  dcterms:identifier "http://anzsoil.org/def/au/asls/land-surface/coarse-fragments-shape-S"^^xsd:anyURI ;
  ui:isMemberOf  <coarse-fragments-shape> ;
  rdfs:comment "C_CF_SHAPE" ;
  rdfs:label "Subangular"@en ;
  skos:definition "Subangular shape as determined from visual guide"@en ;
  skos:inScheme <> ;
  skos:notation "S" ;
  skos:prefLabel "Subangular"@en ;
  skos:topConceptOf <> ;
.
 <coarse-fragments-shape-SP>
  a skos:Concept ;
  dcterms:description "Subangular platy shape as determined from visual guide"@en ;
  dcterms:identifier "http://anzsoil.org/def/au/asls/land-surface/coarse-fragments-shape-SP"^^xsd:anyURI ;
  ui:isMemberOf  <coarse-fragments-shape> ;
  rdfs:comment "C_CF_SHAPE" ;
  rdfs:label "Subangular platy"@en ;
  skos:definition "Subangular platy shape as determined from visual guide"@en ;
  skos:inScheme <> ;
  skos:notation "SP" ;
  skos:prefLabel "Subangular platy"@en ;
  skos:topConceptOf <> ;
.
 <coarse-fragments-shape-ST>
  a skos:Concept ;
  dcterms:description "Subangular tabular shape as determined from visual guide"@en ;
  dcterms:identifier "http://anzsoil.org/def/au/asls/land-surface/coarse-fragments-shape-ST"^^xsd:anyURI ;
  ui:isMemberOf  <coarse-fragments-shape> ;
  rdfs:comment "C_CF_SHAPE" ;
  rdfs:label "Subangular tabular"@en ;
  skos:definition "Subangular tabular shape as determined from visual guide"@en ;
  skos:inScheme <> ;
  skos:notation "ST" ;
  skos:prefLabel "Subangular tabular"@en ;
  skos:topConceptOf <> ;
.
 <coarse-fragments-shape-U>
  a skos:Concept ;
  dcterms:description "Subrounded shape as determined from visual guide"@en ;
  dcterms:identifier "http://anzsoil.org/def/au/asls/land-surface/coarse-fragments-shape-U"^^xsd:anyURI ;
  ui:isMemberOf  <coarse-fragments-shape> ;
  rdfs:comment "C_CF_SHAPE" ;
  rdfs:label "Subrounded"@en ;
  skos:definition "Subrounded shape as determined from visual guide"@en ;
  skos:inScheme <> ;
  skos:notation "U" ;
  skos:prefLabel "Subrounded"@en ;
  skos:topConceptOf <> ;
.
 <coarse-fragments-shape-UP>
  a skos:Concept ;
  dcterms:description "Subrounded platy shape as determined from visual guide"@en ;
  dcterms:identifier "http://anzsoil.org/def/au/asls/land-surface/coarse-fragments-shape-UP"^^xsd:anyURI ;
  ui:isMemberOf  <coarse-fragments-shape> ;
  rdfs:comment "C_CF_SHAPE" ;
  rdfs:label "Subrounded platy"@en ;
  skos:definition "Subrounded platy shape as determined from visual guide"@en ;
  skos:inScheme <> ;
  skos:notation "UP" ;
  skos:prefLabel "Subrounded platy"@en ;
  skos:topConceptOf <> ;
.
 <coarse-fragments-shape-UT>
  a skos:Concept ;
  dcterms:description "Subrounded tabular shape as determined from visual guide"@en ;
  dcterms:identifier "http://anzsoil.org/def/au/asls/land-surface/coarse-fragments-shape-UT"^^xsd:anyURI ;
  ui:isMemberOf  <coarse-fragments-shape> ;
  rdfs:comment "C_CF_SHAPE" ;
  rdfs:label "Subrounded tabular"@en ;
  skos:definition "Subrounded tabular shape as determined from visual guide"@en ;
  skos:inScheme <> ;
  skos:notation "UT" ;
  skos:prefLabel "Subrounded tabular"@en ;
  skos:topConceptOf <> ;
.
 <coarse-fragments-size>
  a skos:Collection ;
  a sosa:ObservableProperty ;
  dcterms:description "The scale adopted employs class boundaries at (2 × 10n/2) mm, where n is an integer. This system is an extension of that used for particles smaller than 2 mm both in the scheme of the British Standards Institution and the Massachusetts Institute of Technology and the original Atterberg (1905) scheme on which the International Scheme was based. It is thus compatible with both the International Scheme referred to in the field texture section and the grain size criteria for substrate materials."@en ;
  dcterms:identifier "http://anzsoil.org/def/au/asls/land-surface/coarse-fragments-size"^^xsd:anyURI ;
  ui:isMemberOf  <coarse-fragments> ;
  rdfs:comment "The terms used to describe size apply to fragments of any shape: The average maximum dimension of fragments is used to determine the class interval. N_CF_SIZE"@en ;
  rdfs:label "Size of coarse fragments"@en ;
  skos:definition "The scale adopted employs class boundaries at (2 × 10n/2) mm, where n is an integer. This system is an extension of that used for particles smaller than 2 mm both in the scheme of the British Standards Institution and the Massachusetts Institute of Technology and the original Atterberg (1905) scheme on which the International Scheme was based. It is thus compatible with both the International Scheme referred to in the field texture section and the grain size criteria for substrate materials."@en ;
  skos:member  <coarse-fragments-size-1> ;
  skos:member  <coarse-fragments-size-2> ;
  skos:member  <coarse-fragments-size-3> ;
  skos:member  <coarse-fragments-size-4> ;
  skos:member  <coarse-fragments-size-5> ;
  skos:member  <coarse-fragments-size-6> ;
  skos:member  <coarse-fragments-size-7> ;
  skos:note "Note that in preparing soils for laboratory analysis, the greater than 2mm size fraction is commonly recorded as 'gravel'."@en ;
  skos:prefLabel "Size of coarse fragments"@en ;
.
 <coarse-fragments-size-1>
  a skos:Concept ;
  dcterms:description "2-6 mm"@en ;
  dcterms:identifier "http://anzsoil.org/def/au/asls/land-surface/coarse-fragments-size-1"^^xsd:anyURI ;
  ui:isMemberOf  <coarse-fragments-size> ;
  rdfs:comment "The terms used to describe size apply to fragments of any shape: The average maximum dimension of fragments is used to determine the class interval. N_CF_SIZE"@en ;
  rdfs:label "Fine gravelly or small pebbles"@en ;
  skos:definition "2-6 mm"@en ;
  skos:inScheme <> ;
  skos:notation "1" ;
  skos:prefLabel "Fine gravelly or small pebbles"@en ;
  skos:topConceptOf <> ;
.
 <coarse-fragments-size-2>
  a skos:Concept ;
  dcterms:description "6-20 mm"@en ;
  dcterms:identifier "http://anzsoil.org/def/au/asls/land-surface/coarse-fragments-size-2"^^xsd:anyURI ;
  ui:isMemberOf  <coarse-fragments-size> ;
  rdfs:comment "The terms used to describe size apply to fragments of any shape: The average maximum dimension of fragments is used to determine the class interval. N_CF_SIZE"@en ;
  rdfs:label "Medium gravelly or medium pebbles"@en ;
  skos:definition "6-20 mm"@en ;
  skos:inScheme <> ;
  skos:notation "2" ;
  skos:prefLabel "Medium gravelly or medium pebbles"@en ;
  skos:topConceptOf <> ;
.
 <coarse-fragments-size-3>
  a skos:Concept ;
  dcterms:description "20-60 mm"@en ;
  dcterms:identifier "http://anzsoil.org/def/au/asls/land-surface/coarse-fragments-size-3"^^xsd:anyURI ;
  ui:isMemberOf  <coarse-fragments-size> ;
  rdfs:comment "The terms used to describe size apply to fragments of any shape: The average maximum dimension of fragments is used to determine the class interval.  N_CF_SIZE"@en ;
  rdfs:label "Coarse gravelly or large pebbles"@en ;
  skos:definition "20-60 mm"@en ;
  skos:inScheme <> ;
  skos:notation "3" ;
  skos:prefLabel "Coarse gravelly or large pebbles"@en ;
  skos:topConceptOf <> ;
.
 <coarse-fragments-size-4>
  a skos:Concept ;
  dcterms:description "60-200 mm"@en ;
  dcterms:identifier "http://anzsoil.org/def/au/asls/land-surface/coarse-fragments-size-4"^^xsd:anyURI ;
  ui:isMemberOf  <coarse-fragments-size> ;
  rdfs:comment "The terms used to describe size apply to fragments of any shape: The average maximum dimension of fragments is used to determine the class interval. N_CF_SIZE"@en ;
  rdfs:label "Cobbly or cobbles"@en ;
  skos:definition "60-200 mm"@en ;
  skos:inScheme <> ;
  skos:notation "4" ;
  skos:prefLabel "Cobbly or cobbles"@en ;
  skos:topConceptOf <> ;
.
 <coarse-fragments-size-5>
  a skos:Concept ;
  dcterms:description "200-600 mm"@en ;
  dcterms:identifier "http://anzsoil.org/def/au/asls/land-surface/coarse-fragments-size-5"^^xsd:anyURI ;
  ui:isMemberOf  <coarse-fragments-size> ;
  rdfs:comment "The terms used to describe size apply to fragments of any shape: The average maximum dimension of fragments is used to determine the class interval. N_CF_SIZE"@en ;
  rdfs:label "Stony or stones"@en ;
  skos:definition "200-600 mm"@en ;
  skos:inScheme <> ;
  skos:notation "5" ;
  skos:prefLabel "Stony or stones"@en ;
  skos:topConceptOf <> ;
.
 <coarse-fragments-size-6>
  a skos:Concept ;
  dcterms:description "600-2000 mm"@en ;
  dcterms:identifier "http://anzsoil.org/def/au/asls/land-surface/coarse-fragments-size-6"^^xsd:anyURI ;
  ui:isMemberOf  <coarse-fragments-size> ;
  rdfs:comment "The terms used to describe size apply to fragments of any shape: The average maximum dimension of fragments is used to determine the class interval. N_CF_SIZE"@en ;
  rdfs:label "Bouldery or boulders"@en ;
  skos:definition "600-2000 mm"@en ;
  skos:inScheme <> ;
  skos:notation "6" ;
  skos:prefLabel "Bouldery or boulders"@en ;
  skos:topConceptOf <> ;
.
 <coarse-fragments-size-7>
  a skos:Concept ;
  dcterms:description ">2000 mm"@en ;
  dcterms:identifier "http://anzsoil.org/def/au/asls/land-surface/coarse-fragments-size-7"^^xsd:anyURI ;
  ui:isMemberOf  <coarse-fragments-size> ;
  rdfs:comment "The terms used to describe size apply to fragments of any shape: The average maximum dimension of fragments is used to determine the class interval. N_CF_SIZE"@en ;
  rdfs:label "Large boulders"@en ;
  skos:definition ">2000 mm"@en ;
  skos:inScheme <> ;
  skos:notation "7" ;
  skos:prefLabel "Large boulders"@en ;
  skos:topConceptOf <> ;
.
 <coarse-fragments-strength>
  a skos:Collection ;
  a sosa:ObservableProperty ;
  dcterms:description "Strength of coarse fragments is the same as for 'Strength of material. The strength of a specimen of soil substrate material may be crudely estimated in the field by striking it with the head-end or the pick-end of a geological hammer or by trying to cut it with a knife, and then referring to Table 32 (ASLS Field Handbook). These estimates refer to the unconfined (or uniaxial) compressive strength. The strength is that of the intact material rather than that of the mass, the strength of which has generally been reduced by the development of fractures and other phenomena."@en ;
  dcterms:identifier "http://anzsoil.org/def/au/asls/land-surface/coarse-fragments-strength"^^xsd:anyURI ;
  ui:isMemberOf  <coarse-fragments> ;
  rdfs:comment "C_CF_STRENGTH"@en ;
  rdfs:label "Strength of coarse fragments"@en ;
  skos:altLabel "Strength of material"@en ;
  skos:definition "Strength of coarse fragments is the same as for 'Strength of material. The strength of a specimen of soil substrate material may be crudely estimated in the field by striking it with the head-end or the pick-end of a geological hammer or by trying to cut it with a knife, and then referring to Table 32 (ASLS Field Handbook). These estimates refer to the unconfined (or uniaxial) compressive strength. The strength is that of the intact material rather than that of the mass, the strength of which has generally been reduced by the development of fractures and other phenomena."@en ;
  skos:exactMatch  <../substrate/material-strength> ;
  skos:member  <../substrate/material-strength-M> ;
  skos:member  <../substrate/material-strength-S> ;
  skos:member  <../substrate/material-strength-VS> ;
  skos:member  <../substrate/material-strength-VW> ;
  skos:member  <../substrate/material-strength-W> ;
  skos:prefLabel "Strength of coarse fragments"@en ;
.
 <depth-free-water>
  a skos:Collection ;
  a sosa:ObservableProperty ;
  dcterms:description "Give depth to free water at the site of soil observation, in metres, either above or below the soil surface, excluding litter and living vegetation. "@en ;
  dcterms:identifier "http://anzsoil.org/def/au/asls/land-surface/depth-free-water"^^xsd:anyURI ;
  ui:topMemberOf <> ;
  rdfs:label "Depth to free water"@en ;
  skos:definition "Give depth to free water at the site of soil observation, in metres, either above or below the soil surface, excluding litter and living vegetation. "@en ;
  skos:member  <depth-free-water-0> ;
  skos:member  <depth-free-water-above> ;
  skos:member  <depth-free-water-below> ;
  skos:prefLabel "Depth to free water"@en ;
.
 <depth-free-water-0>
  a skos:Concept ;
  dcterms:description "If there is no free water, record:"@en ;
  dcterms:identifier "http://anzsoil.org/def/au/asls/land-surface/depth-free-water-0"^^xsd:anyURI ;
  ui:isMemberOf  <depth-free-water> ;
  rdfs:label "No free water"@en ;
  skos:definition "If there is no free water, record:"@en ;
  skos:inScheme <> ;
  skos:notation "0" ;
  skos:prefLabel "No free water"@en ;
  skos:topConceptOf <> ;
.
 <depth-free-water-above>
  a skos:Concept ;
  dcterms:description "Above soil surface."@en ;
  dcterms:identifier "http://anzsoil.org/def/au/asls/land-surface/depth-free-water-above"^^xsd:anyURI ;
  ui:isMemberOf  <depth-free-water> ;
  rdfs:label "Above soil surface"@en ;
  skos:definition "Above soil surface."@en ;
  skos:inScheme <> ;
  skos:notation "+" ;
  skos:prefLabel "Above soil surface"@en ;
  skos:topConceptOf <> ;
.
 <depth-free-water-below>
  a skos:Concept ;
  dcterms:description "Below soil surface."@en ;
  dcterms:identifier "http://anzsoil.org/def/au/asls/land-surface/depth-free-water-below"^^xsd:anyURI ;
  ui:isMemberOf  <depth-free-water> ;
  rdfs:label "Below soil surface"@en ;
  skos:definition "Below soil surface."@en ;
  skos:inScheme <> ;
  skos:notation "-" ;
  skos:prefLabel "Below soil surface"@en ;
  skos:topConceptOf <> ;
.
 <disturbance-of-site>
  a skos:Collection ;
  a sosa:ObservableProperty ;
  dcterms:description "These are broad categories of disturbance. Users may subdivide where considered necessary."@en ;
  dcterms:identifier "http://anzsoil.org/def/au/asls/land-surface/disturbance-of-site"^^xsd:anyURI ;
  ui:topMemberOf <> ;
  rdfs:label "Disturbance of site"@en ;
  skos:definition "These are broad categories of disturbance. Users may subdivide where considered necessary."@en ;
  skos:member  <disturbance-of-site-0> ;
  skos:member  <disturbance-of-site-1> ;
  skos:member  <disturbance-of-site-2> ;
  skos:member  <disturbance-of-site-3> ;
  skos:member  <disturbance-of-site-4> ;
  skos:member  <disturbance-of-site-5> ;
  skos:member  <disturbance-of-site-6> ;
  skos:member  <disturbance-of-site-7> ;
  skos:member  <disturbance-of-site-8> ;
  skos:prefLabel "Disturbance of site"@en ;
.
 <disturbance-of-site-0>
  a skos:Concept ;
  dcterms:description "No effective disturbance; natural."@en ;
  dcterms:identifier "http://anzsoil.org/def/au/asls/land-surface/disturbance-of-site-0"^^xsd:anyURI ;
  ui:isMemberOf  <disturbance-of-site> ;
  rdfs:label "No effective disturbance; natural"@en ;
  skos:definition "No effective disturbance; natural."@en ;
  skos:inScheme <> ;
  skos:notation "0" ;
  skos:prefLabel "No effective disturbance; natural"@en ;
  skos:topConceptOf <> ;
.
 <disturbance-of-site-1>
  a skos:Concept ;
  dcterms:description "No effective disturbance other than grazing by hoofed animals."@en ;
  dcterms:identifier "http://anzsoil.org/def/au/asls/land-surface/disturbance-of-site-1"^^xsd:anyURI ;
  ui:isMemberOf  <disturbance-of-site> ;
  rdfs:label "No effective disturbance other than grazing by hoofed animals"@en ;
  skos:definition "No effective disturbance other than grazing by hoofed animals."@en ;
  skos:inScheme <> ;
  skos:notation "1" ;
  skos:prefLabel "No effective disturbance other than grazing by hoofed animals"@en ;
  skos:topConceptOf <> ;
.
 <disturbance-of-site-2>
  a skos:Concept ;
  dcterms:description "Limited clearing, for example selective logging. "@en ;
  dcterms:identifier "http://anzsoil.org/def/au/asls/land-surface/disturbance-of-site-2"^^xsd:anyURI ;
  ui:isMemberOf  <disturbance-of-site> ;
  rdfs:label "Limited clearing"@en ;
  skos:definition "Limited clearing, for example selective logging."@en ;
  skos:inScheme <> ;
  skos:notation "2" ;
  skos:prefLabel "Limited clearing"@en ;
  skos:topConceptOf <> ;
.
 <disturbance-of-site-3>
  a skos:Concept ;
  dcterms:description "Extensive clearing, for example poisoning, ringbarking. "@en ;
  dcterms:identifier "http://anzsoil.org/def/au/asls/land-surface/disturbance-of-site-3"^^xsd:anyURI ;
  ui:isMemberOf  <disturbance-of-site> ;
  rdfs:label "Extensive clearing"@en ;
  skos:definition "Extensive clearing, for example poisoning, ringbarking."@en ;
  skos:inScheme <> ;
  skos:notation "3" ;
  skos:prefLabel "Extensive clearing"@en ;
  skos:topConceptOf <> ;
.
 <disturbance-of-site-4>
  a skos:Concept ;
  dcterms:description "Complete clearing; pasture, native or improved, but never cultivated. "@en ;
  dcterms:identifier "http://anzsoil.org/def/au/asls/land-surface/disturbance-of-site-4"^^xsd:anyURI ;
  ui:isMemberOf  <disturbance-of-site> ;
  rdfs:label "Complete clearing; pasture, native or improved, but never cultivated"@en ;
  skos:definition "Complete clearing; pasture, native or improved, but never cultivated."@en ;
  skos:inScheme <> ;
  skos:notation "4" ;
  skos:prefLabel "Complete clearing; pasture, native or improved, but never cultivated"@en ;
  skos:topConceptOf <> ;
.
 <disturbance-of-site-5>
  a skos:Concept ;
  dcterms:description "Complete clearing; pasture, native or improved, cultivated at some stage. "@en ;
  dcterms:identifier "http://anzsoil.org/def/au/asls/land-surface/disturbance-of-site-5"^^xsd:anyURI ;
  ui:isMemberOf  <disturbance-of-site> ;
  rdfs:label "Complete clearing; pasture, native or improved, cultivated at some stage"@en ;
  skos:definition "Complete clearing; pasture, native or improved, cultivated at some stage."@en ;
  skos:inScheme <> ;
  skos:notation "5" ;
  skos:prefLabel "Complete clearing; pasture, native or improved, cultivated at some stage"@en ;
  skos:topConceptOf <> ;
.
 <disturbance-of-site-6>
  a skos:Concept ;
  dcterms:description "Cultivation; rainfed. "@en ;
  dcterms:identifier "http://anzsoil.org/def/au/asls/land-surface/disturbance-of-site-6"^^xsd:anyURI ;
  ui:isMemberOf  <disturbance-of-site> ;
  rdfs:label "Cultivation; rainfed"@en ;
  skos:definition "Cultivation; rainfed."@en ;
  skos:inScheme <> ;
  skos:notation "6" ;
  skos:prefLabel "Cultivation; rainfed"@en ;
  skos:topConceptOf <> ;
.
 <disturbance-of-site-7>
  a skos:Concept ;
  dcterms:description "Cultivation; irrigated, past or present. "@en ;
  dcterms:identifier "http://anzsoil.org/def/au/asls/land-surface/disturbance-of-site-7"^^xsd:anyURI ;
  ui:isMemberOf  <disturbance-of-site> ;
  rdfs:label "Cultivation; irrigated, past or present"@en ;
  skos:definition "Cultivation; irrigated, past or present."@en ;
  skos:inScheme <> ;
  skos:notation "7" ;
  skos:prefLabel "Cultivation; irrigated, past or present"@en ;
  skos:topConceptOf <> ;
.
 <disturbance-of-site-8>
  a skos:Concept ;
  dcterms:description "Highly disturbed, for example quarrying, road works, mining, landfill, urban. "@en ;
  dcterms:identifier "http://anzsoil.org/def/au/asls/land-surface/disturbance-of-site-8"^^xsd:anyURI ;
  ui:isMemberOf  <disturbance-of-site> ;
  rdfs:label "Highly disturbed"@en ;
  skos:definition "Highly disturbed, for example quarrying, road works, mining, landfill, urban."@en ;
  skos:inScheme <> ;
  skos:notation "8" ;
  skos:prefLabel "Highly disturbed"@en ;
  skos:topConceptOf <> ;
.
 <drainage-height>
  a skos:Collection ;
  a sosa:ObservableProperty ;
  dcterms:description "This is the height of the point of soil observation above the flat, depression or stream channel that forms the effective bottom of the toposequence. Give drainage height in metres."@en ;
  dcterms:identifier "http://anzsoil.org/def/au/asls/land-surface/drainage-height"^^xsd:anyURI ;
  rdfs:label "Drainage height"@en ;
  skos:definition "This is the height of the point of soil observation above the flat, depression or stream channel that forms the effective bottom of the toposequence. Give drainage height in metres."@en ;
  skos:member  <drainage-height-evaluation-means> ;
  skos:prefLabel "Drainage height"@en ;
.
 <drainage-height-evaluation-means>
  a skos:Collection ;
  dcterms:description "Means of evaluation of drainage height."@en ;
  dcterms:identifier "http://anzsoil.org/def/au/asls/land-surface/drainage-height-evaluation-means"^^xsd:anyURI ;
  ui:isMemberOf  <drainage-height> ;
  rdfs:label "Means of evaluation of drainage height"@en ;
  skos:definition "Means of evaluation of drainage height."@en ;
  skos:member  <drainage-height-evaluation-means-A> ;
  skos:member  <drainage-height-evaluation-means-E> ;
  skos:member  <drainage-height-evaluation-means-L> ;
  skos:member  <drainage-height-evaluation-means-M> ;
  skos:prefLabel "Means of evaluation of drainage height"@en ;
.
 <drainage-height-evaluation-means-A>
  a skos:Concept ;
  dcterms:description "Determined by altimeter"@en ;
  dcterms:identifier "http://anzsoil.org/def/au/asls/land-surface/drainage-height-evaluation-means-A"^^xsd:anyURI ;
  ui:isMemberOf  <drainage-height-evaluation-means> ;
  rdfs:label "Determined by altimeter (drainage height)"@en ;
  skos:definition "Determined by altimeter"@en ;
  skos:exactMatch  <elevation-evaluation-means-A> ;
  skos:inScheme <> ;
  skos:notation "A" ;
  skos:prefLabel "Determined by altimeter (drainage height)"@en ;
  skos:topConceptOf <> ;
.
 <drainage-height-evaluation-means-E>
  a skos:Concept ;
  dcterms:description "Estimate"@en ;
  dcterms:identifier "http://anzsoil.org/def/au/asls/land-surface/drainage-height-evaluation-means-E"^^xsd:anyURI ;
  ui:isMemberOf  <drainage-height-evaluation-means> ;
  rdfs:label "Estimate (drainage height)"@en ;
  skos:definition "Estimate"@en ;
  skos:exactMatch  <elevation-evaluation-means-E> ;
  skos:inScheme <> ;
  skos:notation "E" ;
  skos:prefLabel "Estimate (drainage height)"@en ;
  skos:topConceptOf <> ;
.
 <drainage-height-evaluation-means-L>
  a skos:Concept ;
  dcterms:description "Levelled from survey datum or estimated from contour plan (1:10 000 or larger scale)"@en ;
  dcterms:identifier "http://anzsoil.org/def/au/asls/land-surface/drainage-height-evaluation-means-L"^^xsd:anyURI ;
  ui:isMemberOf  <drainage-height-evaluation-means> ;
  rdfs:label "Levelled from survey datum or estimated from contour plan (drainage height)"@en ;
  skos:definition "Levelled from survey datum or estimated from contour plan (1:10 000 or larger scale)"@en ;
  skos:exactMatch  <elevation-evaluation-means-L> ;
  skos:inScheme <> ;
  skos:notation "L" ;
  skos:prefLabel "Levelled from survey datum or estimated from contour plan (drainage height)"@en ;
  skos:topConceptOf <> ;
.
 <drainage-height-evaluation-means-M>
  a skos:Concept ;
  dcterms:description "Interpolated from contour map with contour interval of 20 m or less"@en ;
  dcterms:identifier "http://anzsoil.org/def/au/asls/land-surface/drainage-height-evaluation-means-M"^^xsd:anyURI ;
  ui:isMemberOf  <drainage-height-evaluation-means> ;
  rdfs:label "Interpolated from contour map (drainage height)"@en ;
  skos:definition "Interpolated from contour map with contour interval of 20 m or less"@en ;
  skos:exactMatch  <elevation-evaluation-means-M> ;
  skos:inScheme <> ;
  skos:notation "M" ;
  skos:prefLabel "Interpolated from contour map (drainage height)"@en ;
  skos:topConceptOf <> ;
.
 <elevation>
  a skos:Collection ;
  a sosa:ObservableProperty ;
  dcterms:description "Give in metres above sea-level."@en ;
  dcterms:identifier "http://anzsoil.org/def/au/asls/land-surface/elevation"^^xsd:anyURI ;
  ui:topMemberOf <> ;
  rdfs:label "Elevation in metres above sea-level"@en ;
  skos:definition "Give in metres above sea-level."@en ;
  skos:member  <elevation-evaluation-means> ;
  skos:prefLabel "Elevation in metres above sea-level"@en ;
.
 <elevation-evaluation-means>
  a skos:Collection ;
  dcterms:description "Means of evaluation of elevation."@en ;
  dcterms:identifier "http://anzsoil.org/def/au/asls/land-surface/elevation-evaluation-means"^^xsd:anyURI ;
  ui:isMemberOf  <elevation> ;
  rdfs:label "Means of evaluation of elevation"@en ;
  skos:definition "Means of evaluation of elevation"@en ;
  skos:member  <elevation-evaluation-means-A> ;
  skos:member  <elevation-evaluation-means-E> ;
  skos:member  <elevation-evaluation-means-L> ;
  skos:member  <elevation-evaluation-means-M> ;
  skos:prefLabel "Means of evaluation of elevation"@en ;
.
 <elevation-evaluation-means-A>
  a skos:Concept ;
  dcterms:description "Determined by altimeter"@en ;
  dcterms:identifier "http://anzsoil.org/def/au/asls/land-surface/elevation-evaluation-means-A"^^xsd:anyURI ;
  ui:isMemberOf  <elevation-evaluation-means> ;
  rdfs:label "Determined by altimeter"@en ;
  skos:definition "Determined by altimeter"@en ;
  skos:exactMatch  <drainage-height-evaluation-means-A> ;
  skos:inScheme <> ;
  skos:notation "A" ;
  skos:prefLabel "Determined by altimeter"@en ;
  skos:topConceptOf <> ;
.
 <elevation-evaluation-means-E>
  a skos:Concept ;
  dcterms:description "Estimate"@en ;
  dcterms:identifier "http://anzsoil.org/def/au/asls/land-surface/elevation-evaluation-means-E"^^xsd:anyURI ;
  ui:isMemberOf  <elevation-evaluation-means> ;
  rdfs:label "Estimate"@en ;
  skos:definition "Estimate"@en ;
  skos:exactMatch  <drainage-height-evaluation-means-E> ;
  skos:inScheme <> ;
  skos:notation "E" ;
  skos:prefLabel "Estimate"@en ;
  skos:topConceptOf <> ;
.
 <elevation-evaluation-means-L>
  a skos:Concept ;
  dcterms:description "Levelled from survey datum or estimated from contour plan (1:10 000 or larger scale)"@en ;
  dcterms:identifier "http://anzsoil.org/def/au/asls/land-surface/elevation-evaluation-means-L"^^xsd:anyURI ;
  ui:isMemberOf  <elevation-evaluation-means> ;
  rdfs:label "Levelled from survey datum or estimated from contour plan"@en ;
  skos:definition "Levelled from survey datum or estimated from contour plan (1:10 000 or larger scale)"@en ;
  skos:exactMatch  <drainage-height-evaluation-means-L> ;
  skos:inScheme <> ;
  skos:notation "L" ;
  skos:prefLabel "Levelled from survey datum or estimated from contour plan"@en ;
  skos:topConceptOf <> ;
.
 <elevation-evaluation-means-M>
  a skos:Concept ;
  dcterms:description "Interpolated from contour map with contour interval of 20 m or less"@en ;
  dcterms:identifier "http://anzsoil.org/def/au/asls/land-surface/elevation-evaluation-means-M"^^xsd:anyURI ;
  ui:isMemberOf  <elevation-evaluation-means> ;
  rdfs:label "Interpolated from contour map"@en ;
  skos:definition "Interpolated from contour map with contour interval of 20 m or less"@en ;
  skos:exactMatch  <drainage-height-evaluation-means-M> ;
  skos:inScheme <> ;
  skos:notation "M" ;
  skos:prefLabel "Interpolated from contour map"@en ;
  skos:topConceptOf <> ;
.
 <erosion>
  a skos:Collection ;
  a sosa:ObservableProperty ;
  dcterms:description """This section is concerned with accelerated erosion rather than natural erosion. Natural or geologic erosion is the type and rate of movement of land surface material in its undisturbed natural environment. Accelerated erosion is the more rapid erosion that follows the destruction or loss of protective cover often resulting from people’s influence on the soil, vegetation or landform. It is not always easy to distinguish between accelerated and natural erosion in some landscapes where both are closely interrelated, nor is it always clear whether wind or water is the dominant agent. This is particularly so in the case of scald formation (Warren 1965).
The complexity of erosion forms creates difficulties in both defining and quantitatively estimating the extent of erosion within the dimensions of the site. Hence, the observer is advised to record the following simple parameters. Assess the erosion observed at the time of the description, not the likelihood of erosion."""@en ;
  dcterms:identifier "http://anzsoil.org/def/au/asls/land-surface/erosion"^^xsd:anyURI ;
  ui:topMemberOf <> ;
  rdfs:comment "For erosion, aggradation and inundation assessment, the extent of the site is 20 m radius."@en ;
  rdfs:label "Erosion"@en ;
  skos:definition """This section is concerned with accelerated erosion rather than natural erosion. Natural or geologic erosion is the type and rate of movement of land surface material in its undisturbed natural environment. Accelerated erosion is the more rapid erosion that follows the destruction or loss of protective cover often resulting from people’s influence on the soil, vegetation or landform. It is not always easy to distinguish between accelerated and natural erosion in some landscapes where both are closely interrelated, nor is it always clear whether wind or water is the dominant agent. This is particularly so in the case of scald formation (Warren 1965).
The complexity of erosion forms creates difficulties in both defining and quantitatively estimating the extent of erosion within the dimensions of the site. Hence, the observer is advised to record the following simple parameters. Assess the erosion observed at the time of the description, not the likelihood of erosion."""@en ;
  skos:member  <erosion-B> ;
  skos:member  <erosion-C> ;
  skos:member  <erosion-G> ;
  skos:member  <erosion-M> ;
  skos:member  <erosion-R> ;
  skos:member  <erosion-S> ;
  skos:member  <erosion-T> ;
  skos:member  <erosion-V> ;
  skos:member  <erosion-W> ;
  skos:member  <erosion-state> ;
  skos:member  <water-erosion> ;
  skos:prefLabel "Erosion"@en ;
.
 <erosion-B>
  a skos:Collection ;
  a sosa:ObservableProperty ;
  dcterms:description "This is the removal of soil from a stream bank, typically during periods of high stream flow."@en ;
  dcterms:identifier "http://anzsoil.org/def/au/asls/land-surface/erosion-B"^^xsd:anyURI ;
  ui:isMemberOf  <erosion> ;
  rdfs:label "Stream bank erosion"@en ;
  skos:definition "This is the removal of soil from a stream bank, typically during periods of high stream flow."@en ;
  skos:member  <erosion-B-0> ;
  skos:member  <erosion-B-1> ;
  skos:member  <erosion-B-X> ;
  skos:notation "B" ;
  skos:prefLabel "Stream bank erosion"@en ;
.
 <erosion-B-0>
  a skos:Concept ;
  dcterms:description "No stream bank erosion."@en ;
  dcterms:identifier "http://anzsoil.org/def/au/asls/land-surface/erosion-B-0"^^xsd:anyURI ;
  ui:isMemberOf  <erosion-B> ;
  rdfs:label "No stream bank erosion"@en ;
  skos:definition "No stream bank erosion."@en ;
  skos:inScheme <> ;
  skos:notation "0" ;
  skos:prefLabel "No stream bank erosion"@en ;
  skos:topConceptOf <> ;
.
 <erosion-B-1>
  a skos:Concept ;
  dcterms:description "Present."@en ;
  dcterms:identifier "http://anzsoil.org/def/au/asls/land-surface/erosion-B-1"^^xsd:anyURI ;
  ui:isMemberOf  <erosion-B> ;
  rdfs:label "Present"@en ;
  skos:definition "Present."@en ;
  skos:inScheme <> ;
  skos:notation "1" ;
  skos:prefLabel "Present"@en ;
  skos:topConceptOf <> ;
.
 <erosion-B-X>
  a skos:Concept ;
  dcterms:description "Not apparent."@en ;
  dcterms:identifier "http://anzsoil.org/def/au/asls/land-surface/erosion-B-X"^^xsd:anyURI ;
  ui:isMemberOf  <erosion-B> ;
  rdfs:label "Not apparent"@en ;
  skos:definition "Not apparent."@en ;
  skos:inScheme <> ;
  skos:notation "X" ;
  skos:prefLabel "Not apparent"@en ;
  skos:topConceptOf <> ;
.
 <erosion-C>
  a skos:Collection ;
  a sosa:ObservableProperty ;
  dcterms:description "This is the removal of surface soil by water and/or wind, often exposing a more clayey subsoil which is devoid of vegetation and relatively impermeable to water. Scalds are most common in arid or semi-arid lands."@en ;
  dcterms:identifier "http://anzsoil.org/def/au/asls/land-surface/erosion-C"^^xsd:anyURI ;
  ui:isMemberOf  <erosion> ;
  rdfs:label "Scald erosion"@en ;
  skos:definition "This is the removal of surface soil by water and/or wind, often exposing a more clayey subsoil which is devoid of vegetation and relatively impermeable to water. Scalds are most common in arid or semi-arid lands."@en ;
  skos:member  <erosion-C-0> ;
  skos:member  <erosion-C-1> ;
  skos:member  <erosion-C-2> ;
  skos:member  <erosion-C-3> ;
  skos:notation "C" ;
  skos:prefLabel "Scald erosion"@en ;
.
 <erosion-C-0>
  a skos:Concept ;
  dcterms:description "No scalding."@en ;
  dcterms:identifier "http://anzsoil.org/def/au/asls/land-surface/erosion-C-0"^^xsd:anyURI ;
  ui:isMemberOf  <erosion-C> ;
  rdfs:label "No scalding"@en ;
  skos:definition "No scalding."@en ;
  skos:inScheme <> ;
  skos:notation "0" ;
  skos:prefLabel "No scalding"@en ;
  skos:topConceptOf <> ;
.
 <erosion-C-1>
  a skos:Concept ;
  dcterms:description "<5% of site scalded."@en ;
  dcterms:identifier "http://anzsoil.org/def/au/asls/land-surface/erosion-C-1"^^xsd:anyURI ;
  ui:isMemberOf  <erosion-C> ;
  rdfs:label "Minor scalding"@en ;
  skos:definition "<5% of site scalded."@en ;
  skos:inScheme <> ;
  skos:notation "1" ;
  skos:prefLabel "Minor scalding"@en ;
  skos:topConceptOf <> ;
.
 <erosion-C-2>
  a skos:Concept ;
  dcterms:description "5-50% of site scalded."@en ;
  dcterms:identifier "http://anzsoil.org/def/au/asls/land-surface/erosion-C-2"^^xsd:anyURI ;
  ui:isMemberOf  <erosion-C> ;
  rdfs:label "Moderate scalding"@en ;
  skos:definition "5-50% of site scalded."@en ;
  skos:inScheme <> ;
  skos:notation "2" ;
  skos:prefLabel "Moderate scalding"@en ;
  skos:topConceptOf <> ;
.
 <erosion-C-3>
  a skos:Concept ;
  dcterms:description ">50% of site scalded."@en ;
  dcterms:identifier "http://anzsoil.org/def/au/asls/land-surface/erosion-C-3"^^xsd:anyURI ;
  ui:isMemberOf  <erosion-C> ;
  rdfs:label "Severe scalding"@en ;
  skos:definition ">50% of site scalded."@en ;
  skos:inScheme <> ;
  skos:notation "3" ;
  skos:prefLabel "Severe scalding"@en ;
  skos:topConceptOf <> ;
.
 <erosion-G>
  a skos:Collection ;
  a sosa:ObservableProperty ;
  dcterms:description "A gully is a channel more than 0.3 m deep."@en ;
  dcterms:identifier "http://anzsoil.org/def/au/asls/land-surface/erosion-G"^^xsd:anyURI ;
  ui:isMemberOf  <erosion> ;
  rdfs:label "Gully erosion"@en ;
  skos:definition "A gully is a channel more than 0.3 m deep."@en ;
  skos:member  <erosion-G-0> ;
  skos:member  <erosion-G-1> ;
  skos:member  <erosion-G-2> ;
  skos:member  <erosion-G-3> ;
  skos:member  <erosion-G-depth> ;
  skos:notation "G" ;
  skos:prefLabel "Gully erosion"@en ;
.
 <erosion-G-0>
  a skos:Concept ;
  dcterms:description "No gully erosion."@en ;
  dcterms:identifier "http://anzsoil.org/def/au/asls/land-surface/erosion-G-0"^^xsd:anyURI ;
  ui:isMemberOf  <erosion-G> ;
  rdfs:label "No gully erosion"@en ;
  skos:definition "No gully erosion."@en ;
  skos:inScheme <> ;
  skos:notation "0" ;
  skos:prefLabel "No gully erosion"@en ;
  skos:topConceptOf <> ;
.
 <erosion-G-1>
  a skos:Concept ;
  dcterms:description "gullies are isolated, linear, discontinuous and restricted to primary or minor drainage lines."@en ;
  dcterms:identifier "http://anzsoil.org/def/au/asls/land-surface/erosion-G-1"^^xsd:anyURI ;
  ui:isMemberOf  <erosion-G> ;
  rdfs:label "Minor gully erosion"@en ;
  skos:definition "gullies are isolated, linear, discontinuous and restricted to primary or minor drainage lines."@en ;
  skos:inScheme <> ;
  skos:notation "1" ;
  skos:prefLabel "Minor gully erosion"@en ;
  skos:topConceptOf <> ;
.
 <erosion-G-2>
  a skos:Concept ;
  dcterms:description "gullies are linear, continuous and restricted to primary and minor drainage lines."@en ;
  dcterms:identifier "http://anzsoil.org/def/au/asls/land-surface/erosion-G-2"^^xsd:anyURI ;
  ui:isMemberOf  <erosion-G> ;
  rdfs:label "Moderate gully erosion"@en ;
  skos:definition "gullies are linear, continuous and restricted to primary and minor drainage lines."@en ;
  skos:inScheme <> ;
  skos:notation "2" ;
  skos:prefLabel "Moderate gully erosion"@en ;
  skos:topConceptOf <> ;
.
 <erosion-G-3>
  a skos:Concept ;
  dcterms:description "gullies are continuous or discontinuous and either tend to branch away from primary drainage lines and on to footslopes, or have multiple branches within primary drainage lines."@en ;
  dcterms:identifier "http://anzsoil.org/def/au/asls/land-surface/erosion-G-3"^^xsd:anyURI ;
  ui:isMemberOf  <erosion-G> ;
  rdfs:label "Severe gully erosion"@en ;
  skos:definition "gullies are continuous or discontinuous and either tend to branch away from primary drainage lines and on to footslopes, or have multiple branches within primary drainage lines."@en ;
  skos:inScheme <> ;
  skos:notation "3" ;
  skos:prefLabel "Severe gully erosion"@en ;
  skos:topConceptOf <> ;
.
 <erosion-G-depth>
  a skos:Collection ;
  dcterms:description "This gives the maximum depth within the site."@en ;
  dcterms:identifier "http://anzsoil.org/def/au/asls/land-surface/erosion-G-depth"^^xsd:anyURI ;
  ui:isMemberOf  <erosion-G> ;
  rdfs:label "Gully depth"@en ;
  skos:definition "This gives the maximum depth within the site."@en ;
  skos:member  <erosion-G-depth-1> ;
  skos:member  <erosion-G-depth-2> ;
  skos:member  <erosion-G-depth-3> ;
  skos:prefLabel "Gully depth"@en ;
.
 <erosion-G-depth-1>
  a skos:Concept ;
  dcterms:description "<1.5 m"@en ;
  dcterms:identifier "http://anzsoil.org/def/au/asls/land-surface/erosion-G-depth-1"^^xsd:anyURI ;
  ui:isMemberOf  <erosion-G-depth> ;
  rdfs:label "Gully depth <1.5 m"@en ;
  skos:definition "<1.5 m"@en ;
  skos:inScheme <> ;
  skos:notation "1" ;
  skos:prefLabel "Gully depth <1.5 m"@en ;
  skos:topConceptOf <> ;
.
 <erosion-G-depth-2>
  a skos:Concept ;
  dcterms:description "1.5-3.0 m"@en ;
  dcterms:identifier "http://anzsoil.org/def/au/asls/land-surface/erosion-G-depth-2"^^xsd:anyURI ;
  ui:isMemberOf  <erosion-G-depth> ;
  rdfs:label "Gully depth 1.5-3.0 m"@en ;
  skos:definition "1.5-3.0 m"@en ;
  skos:inScheme <> ;
  skos:notation "2" ;
  skos:prefLabel "Gully depth 1.5-3.0 m"@en ;
  skos:topConceptOf <> ;
.
 <erosion-G-depth-3>
  a skos:Concept ;
  dcterms:description ">3 m"@en ;
  dcterms:identifier "http://anzsoil.org/def/au/asls/land-surface/erosion-G-depth-3"^^xsd:anyURI ;
  ui:isMemberOf  <erosion-G-depth> ;
  rdfs:label "Gully depth >3 m"@en ;
  skos:definition ">3 m"@en ;
  skos:inScheme <> ;
  skos:notation "3" ;
  skos:prefLabel "Gully depth >3 m"@en ;
  skos:topConceptOf <> ;
.
 <erosion-M>
  a skos:Collection ;
  a sosa:ObservableProperty ;
  dcterms:description "This includes all relatively large downslope movement of soil, rock or mixture of both, for example landslides, slumps, earth flows, debris avalanches and solifluxion."@en ;
  dcterms:identifier "http://anzsoil.org/def/au/asls/land-surface/erosion-M"^^xsd:anyURI ;
  ui:isMemberOf  <erosion> ;
  rdfs:label "Mass movement"@en ;
  skos:definition "This includes all relatively large downslope movement of soil, rock or mixture of both, for example landslides, slumps, earth flows, debris avalanches and solifluxion."@en ;
  skos:member  <erosion-M-0> ;
  skos:member  <erosion-M-1> ;
  skos:notation "M" ;
  skos:prefLabel "Mass movement"@en ;
.
 <erosion-M-0>
  a skos:Concept ;
  dcterms:description "No mass movement."@en ;
  dcterms:identifier "http://anzsoil.org/def/au/asls/land-surface/erosion-M-0"^^xsd:anyURI ;
  ui:isMemberOf  <erosion-M> ;
  rdfs:label "No mass movement"@en ;
  skos:definition "No mass movement."@en ;
  skos:inScheme <> ;
  skos:notation "0" ;
  skos:prefLabel "No mass movement"@en ;
  skos:topConceptOf <> ;
.
 <erosion-M-1>
  a skos:Concept ;
  dcterms:description "Present."@en ;
  dcterms:identifier "http://anzsoil.org/def/au/asls/land-surface/erosion-M-1"^^xsd:anyURI ;
  ui:isMemberOf  <erosion-M> ;
  rdfs:label "Present"@en ;
  skos:definition "Present."@en ;
  skos:inScheme <> ;
  skos:notation "1" ;
  skos:prefLabel "Present"@en ;
  skos:topConceptOf <> ;
.
 <erosion-R>
  a skos:Collection ;
  a sosa:ObservableProperty ;
  dcterms:description "A rill is a small channel up to 0.3 m deep, which can be largely obliterated by tillage operations (Houghton and Charman 1986)."@en ;
  dcterms:identifier "http://anzsoil.org/def/au/asls/land-surface/erosion-R"^^xsd:anyURI ;
  ui:isMemberOf  <erosion> ;
  rdfs:label "Rill erosion"@en ;
  skos:definition "A rill is a small channel up to 0.3 m deep, which can be largely obliterated by tillage operations (Houghton and Charman 1986)."@en ;
  skos:member  <erosion-R-0> ;
  skos:member  <erosion-R-1> ;
  skos:member  <erosion-R-2> ;
  skos:member  <erosion-R-3> ;
  skos:notation "R" ;
  skos:prefLabel "Rill erosion"@en ;
.
 <erosion-R-0>
  a skos:Concept ;
  dcterms:description "no rill erosion."@en ;
  dcterms:identifier "http://anzsoil.org/def/au/asls/land-surface/erosion-R-0"^^xsd:anyURI ;
  ui:isMemberOf  <erosion-R> ;
  rdfs:label "No rill erosion"@en ;
  skos:definition "no rill erosion."@en ;
  skos:inScheme <> ;
  skos:notation "0" ;
  skos:prefLabel "No rill erosion"@en ;
  skos:topConceptOf <> ;
.
 <erosion-R-1>
  a skos:Concept ;
  dcterms:description "occasional rills."@en ;
  dcterms:identifier "http://anzsoil.org/def/au/asls/land-surface/erosion-R-1"^^xsd:anyURI ;
  ui:isMemberOf  <erosion-R> ;
  rdfs:label "Minor"@en ;
  skos:definition "occasional rills."@en ;
  skos:inScheme <> ;
  skos:notation "1" ;
  skos:prefLabel "Minor"@en ;
  skos:topConceptOf <> ;
.
 <erosion-R-2>
  a skos:Concept ;
  dcterms:description "common rills."@en ;
  dcterms:identifier "http://anzsoil.org/def/au/asls/land-surface/erosion-R-2"^^xsd:anyURI ;
  ui:isMemberOf  <erosion-R> ;
  rdfs:label "Moderate"@en ;
  skos:definition "common rills."@en ;
  skos:inScheme <> ;
  skos:notation "2" ;
  skos:prefLabel "Moderate"@en ;
  skos:topConceptOf <> ;
.
 <erosion-R-3>
  a skos:Concept ;
  dcterms:description "numerous rills forming corrugated ground surface."@en ;
  dcterms:identifier "http://anzsoil.org/def/au/asls/land-surface/erosion-R-3"^^xsd:anyURI ;
  ui:isMemberOf  <erosion-R> ;
  rdfs:label "Severe"@en ;
  skos:definition "numerous rills forming corrugated ground surface."@en ;
  skos:inScheme <> ;
  skos:notation "3" ;
  skos:prefLabel "Severe"@en ;
  skos:topConceptOf <> ;
.
 <erosion-S>
  a skos:Collection ;
  a sosa:ObservableProperty ;
  dcterms:description "This is the relatively uniform removal of soil from an area without the development of conspicuous channels. Indicators of sheet erosion include soil deposits in downslope sediment traps, such as fencelines or farm dams, and pedestalling, root exposure or exposure of subsoils."@en ;
  dcterms:identifier "http://anzsoil.org/def/au/asls/land-surface/erosion-S"^^xsd:anyURI ;
  ui:isMemberOf  <erosion> ;
  rdfs:label "Sheet erosion"@en ;
  skos:definition "This is the relatively uniform removal of soil from an area without the development of conspicuous channels. Indicators of sheet erosion include soil deposits in downslope sediment traps, such as fencelines or farm dams, and pedestalling, root exposure or exposure of subsoils."@en ;
  skos:member  <erosion-S-0> ;
  skos:member  <erosion-S-1> ;
  skos:member  <erosion-S-2> ;
  skos:member  <erosion-S-3> ;
  skos:member  <erosion-S-X> ;
  skos:notation "S" ;
  skos:prefLabel "Sheet erosion"@en ;
.
 <erosion-S-0>
  a skos:Concept ;
  dcterms:description "no sheet erosion."@en ;
  dcterms:identifier "http://anzsoil.org/def/au/asls/land-surface/erosion-S-0"^^xsd:anyURI ;
  ui:isMemberOf  <erosion-S> ;
  rdfs:label "No sheet erosion"@en ;
  skos:definition "no sheet erosion."@en ;
  skos:inScheme <> ;
  skos:notation "0" ;
  skos:prefLabel "No sheet erosion"@en ;
  skos:topConceptOf <> ;
.
 <erosion-S-1>
  a skos:Concept ;
  dcterms:description "indicators may include shallow soil deposits in downslope sediment traps (fencelines, farm dams). Often very difficult to assess as evidence may be lost with cultivation, pedo-turbation or revegetation."@en ;
  dcterms:identifier "http://anzsoil.org/def/au/asls/land-surface/erosion-S-1"^^xsd:anyURI ;
  ui:isMemberOf  <erosion-S> ;
  rdfs:label "Minor"@en ;
  skos:definition "indicators may include shallow soil deposits in downslope sediment traps (fencelines, farm dams). Often very difficult to assess as evidence may be lost with cultivation, pedo-turbation or revegetation."@en ;
  skos:inScheme <> ;
  skos:notation "1" ;
  skos:prefLabel "Minor"@en ;
  skos:topConceptOf <> ;
.
 <erosion-S-2>
  a skos:Concept ;
  dcterms:description "indicators may include partial exposure of roots, moderate soil deposits in downslope sediment traps (fencelines, farm dams)."@en ;
  dcterms:identifier "http://anzsoil.org/def/au/asls/land-surface/erosion-S-2"^^xsd:anyURI ;
  ui:isMemberOf  <erosion-S> ;
  rdfs:label "Moderate"@en ;
  skos:definition "indicators may include partial exposure of roots, moderate soil deposits in downslope sediment traps (fencelines, farm dams)."@en ;
  skos:inScheme <> ;
  skos:notation "2" ;
  skos:prefLabel "Moderate"@en ;
  skos:topConceptOf <> ;
.
 <erosion-S-3>
  a skos:Concept ;
  dcterms:description "indicators may include loss of surface horizons, exposure of subsoil horizons, pedestalling, root exposure, substantial soil deposits in downslope sediment traps (fencelines, farm dams)."@en ;
  dcterms:identifier "http://anzsoil.org/def/au/asls/land-surface/erosion-S-3"^^xsd:anyURI ;
  ui:isMemberOf  <erosion-S> ;
  rdfs:label "Severe"@en ;
  skos:definition "indicators may include loss of surface horizons, exposure of subsoil horizons, pedestalling, root exposure, substantial soil deposits in downslope sediment traps (fencelines, farm dams)."@en ;
  skos:inScheme <> ;
  skos:notation "3" ;
  skos:prefLabel "Severe"@en ;
  skos:topConceptOf <> ;
.
 <erosion-S-X>
  a skos:Concept ;
  dcterms:description "not apparent."@en ;
  dcterms:identifier "http://anzsoil.org/def/au/asls/land-surface/erosion-S-X"^^xsd:anyURI ;
  ui:isMemberOf  <erosion-S> ;
  rdfs:label "Not apparent"@en ;
  skos:definition "not apparent."@en ;
  skos:inScheme <> ;
  skos:notation "X" ;
  skos:prefLabel "Not apparent"@en ;
  skos:topConceptOf <> ;
.
 <erosion-T>
  a skos:Collection ;
  a sosa:ObservableProperty ;
  dcterms:description "This is the removal of subsoil by water while the surface soil remains relatively intact (Crouch 1976)."@en ;
  dcterms:identifier "http://anzsoil.org/def/au/asls/land-surface/erosion-T"^^xsd:anyURI ;
  ui:isMemberOf  <erosion> ;
  rdfs:label "Tunnel erosion"@en ;
  skos:definition "This is the removal of subsoil by water while the surface soil remains relatively intact (Crouch 1976)."@en ;
  skos:member  <erosion-T-0> ;
  skos:member  <erosion-T-1> ;
  skos:member  <erosion-T-X> ;
  skos:notation "T" ;
  skos:prefLabel "Tunnel erosion"@en ;
.
 <erosion-T-0>
  a skos:Concept ;
  dcterms:description "no tunnel erosion."@en ;
  dcterms:identifier "http://anzsoil.org/def/au/asls/land-surface/erosion-T-0"^^xsd:anyURI ;
  ui:isMemberOf  <erosion> ;
  ui:isMemberOf  <erosion-T> ;
  rdfs:label "No tunnel erosion"@en ;
  skos:definition "no tunnel erosion."@en ;
  skos:inScheme <> ;
  skos:notation "0" ;
  skos:prefLabel "No tunnel erosion"@en ;
  skos:topConceptOf <> ;
.
 <erosion-T-1>
  a skos:Concept ;
  dcterms:description "present."@en ;
  dcterms:identifier "http://anzsoil.org/def/au/asls/land-surface/erosion-T-1"^^xsd:anyURI ;
  ui:isMemberOf  <erosion-T> ;
  rdfs:label "Present"@en ;
  skos:definition "present."@en ;
  skos:inScheme <> ;
  skos:notation "1" ;
  skos:prefLabel "Present"@en ;
  skos:topConceptOf <> ;
.
 <erosion-T-X>
  a skos:Concept ;
  dcterms:description "Not apparent."@en ;
  dcterms:identifier "http://anzsoil.org/def/au/asls/land-surface/erosion-T-X"^^xsd:anyURI ;
  ui:isMemberOf  <erosion-T> ;
  rdfs:label "Not apparent"@en ;
  skos:definition "Not apparent."@en ;
  skos:inScheme <> ;
  skos:notation "X" ;
  skos:prefLabel "Not apparent"@en ;
  skos:topConceptOf <> ;
.
 <erosion-V>
  a skos:Collection ;
  a sosa:ObservableProperty ;
  dcterms:description "Erosion of beaches, beach ridges and/or dunes. This is the removal of sand or soil from the margins of beaches, beach ridges, dunes, lakes or dams by wave action."@en ;
  dcterms:identifier "http://anzsoil.org/def/au/asls/land-surface/erosion-V"^^xsd:anyURI ;
  ui:isMemberOf  <erosion> ;
  rdfs:label "Wave erosion"@en ;
  skos:definition "Erosion of beaches, beach ridges and/or dunes. This is the removal of sand or soil from the margins of beaches, beach ridges, dunes, lakes or dams by wave action."@en ;
  skos:member  <erosion-V-0> ;
  skos:member  <erosion-V-1> ;
  skos:member  <erosion-V-X> ;
  skos:notation "V" ;
  skos:prefLabel "Wave erosion"@en ;
.
 <erosion-V-0>
  a skos:Concept ;
  dcterms:description "no wave erosion."@en ;
  dcterms:identifier "http://anzsoil.org/def/au/asls/land-surface/erosion-V-0"^^xsd:anyURI ;
  ui:isMemberOf  <erosion-V> ;
  rdfs:label "No wave erosion"@en ;
  skos:definition "no wave erosion."@en ;
  skos:inScheme <> ;
  skos:notation "0" ;
  skos:prefLabel "No wave erosion"@en ;
  skos:topConceptOf <> ;
.
 <erosion-V-1>
  a skos:Concept ;
  dcterms:description "present."@en ;
  dcterms:identifier "http://anzsoil.org/def/au/asls/land-surface/erosion-V-1"^^xsd:anyURI ;
  ui:isMemberOf  <erosion-V> ;
  rdfs:label "Present"@en ;
  skos:definition "present."@en ;
  skos:inScheme <> ;
  skos:notation "1" ;
  skos:prefLabel "Present"@en ;
  skos:topConceptOf <> ;
.
 <erosion-V-X>
  a skos:Concept ;
  dcterms:description "Not apparent."@en ;
  dcterms:identifier "http://anzsoil.org/def/au/asls/land-surface/erosion-V-X"^^xsd:anyURI ;
  ui:isMemberOf  <erosion-V> ;
  rdfs:label "Not apparent"@en ;
  skos:definition "Not apparent."@en ;
  skos:inScheme <> ;
  skos:notation "X" ;
  skos:prefLabel "Not apparent"@en ;
  skos:topConceptOf <> ;
.
 <erosion-W>
  a skos:Collection ;
  a sosa:ObservableProperty ;
  dcterms:description "Give presence/absence or extent of accelerated erosion."@en ;
  dcterms:identifier "http://anzsoil.org/def/au/asls/land-surface/erosion-W"^^xsd:anyURI ;
  ui:isMemberOf  <erosion> ;
  rdfs:label "Wind erosion"@en ;
  skos:definition "Give presence/absence or extent of accelerated erosion."@en ;
  skos:member  <erosion-W-0> ;
  skos:member  <erosion-W-1> ;
  skos:member  <erosion-W-2> ;
  skos:member  <erosion-W-3> ;
  skos:member  <erosion-W-4> ;
  skos:member  <erosion-W-X> ;
  skos:notation "W" ;
  skos:prefLabel "Wind erosion"@en ;
.
 <erosion-W-0>
  a skos:Concept ;
  dcterms:description "no wind erosion."@en ;
  dcterms:identifier "http://anzsoil.org/def/au/asls/land-surface/erosion-W-0"^^xsd:anyURI ;
  ui:isMemberOf  <erosion-W> ;
  rdfs:label "No wind erosion"@en ;
  skos:definition "no wind erosion."@en ;
  skos:inScheme <> ;
  skos:notation "0" ;
  skos:prefLabel "No wind erosion"@en ;
  skos:topConceptOf <> ;
.
 <erosion-W-1>
  a skos:Concept ;
  dcterms:description "some loss of surface."@en ;
  dcterms:identifier "http://anzsoil.org/def/au/asls/land-surface/erosion-W-1"^^xsd:anyURI ;
  ui:isMemberOf  <erosion-W> ;
  rdfs:label "Minor or present"@en ;
  skos:definition "some loss of surface."@en ;
  skos:inScheme <> ;
  skos:notation "1" ;
  skos:prefLabel "Minor or present"@en ;
  skos:topConceptOf <> ;
.
 <erosion-W-2>
  a skos:Concept ;
  dcterms:description "most or all or surface removed leaving soft or loose material."@en ;
  dcterms:identifier "http://anzsoil.org/def/au/asls/land-surface/erosion-W-2"^^xsd:anyURI ;
  ui:isMemberOf  <erosion-W> ;
  rdfs:label "Moderate"@en ;
  skos:definition "most or all or surface removed leaving soft or loose material."@en ;
  skos:inScheme <> ;
  skos:notation "2" ;
  skos:prefLabel "Moderate"@en ;
  skos:topConceptOf <> ;
.
 <erosion-W-3>
  a skos:Concept ;
  dcterms:description "most or all of surface removed, leaving hard material."@en ;
  dcterms:identifier "http://anzsoil.org/def/au/asls/land-surface/erosion-W-3"^^xsd:anyURI ;
  ui:isMemberOf  <erosion-W> ;
  rdfs:label "Severe"@en ;
  skos:definition "most or all of surface removed, leaving hard material."@en ;
  skos:inScheme <> ;
  skos:notation "3" ;
  skos:prefLabel "Severe"@en ;
  skos:topConceptOf <> ;
.
 <erosion-W-4>
  a skos:Concept ;
  dcterms:description "deeper layers exposed, leaving hard material, for example subsoil, weathered country rock or pans."@en ;
  dcterms:identifier "http://anzsoil.org/def/au/asls/land-surface/erosion-W-4"^^xsd:anyURI ;
  ui:isMemberOf  <erosion-W> ;
  rdfs:label "Very severe"@en ;
  skos:definition "deeper layers exposed, leaving hard material, for example subsoil, weathered country rock or pans."@en ;
  skos:inScheme <> ;
  skos:notation "4" ;
  skos:prefLabel "Very severe"@en ;
  skos:topConceptOf <> ;
.
 <erosion-W-X>
  a skos:Concept ;
  dcterms:description "Not apparent."@en ;
  dcterms:identifier "http://anzsoil.org/def/au/asls/land-surface/erosion-W-X"^^xsd:anyURI ;
  ui:isMemberOf  <erosion-W> ;
  rdfs:label "Not apparent"@en ;
  skos:definition "Not apparent."@en ;
  skos:inScheme <> ;
  skos:notation "X" ;
  skos:prefLabel "Not apparent"@en ;
  skos:topConceptOf <> ;
.
 <erosion-state>
  a skos:Collection ;
  a sosa:ObservableProperty ;
  dcterms:description "State of erosion"@en ;
  dcterms:identifier "http://anzsoil.org/def/au/asls/land-surface/erosion-state"^^xsd:anyURI ;
  ui:isMemberOf  <erosion> ;
  rdfs:label "State of erosion"@en ;
  skos:definition "State of erosion"@en ;
  skos:member  <erosion-state-A> ;
  skos:member  <erosion-state-P> ;
  skos:member  <erosion-state-S> ;
  skos:prefLabel "State of erosion"@en ;
.
 <erosion-state-A>
  a skos:Concept ;
  dcterms:description "one or both of the following conditions apply: evidence of sediment movement; sides and/or floors of erosion form are relatively bare of vegetation."@en ;
  dcterms:identifier "http://anzsoil.org/def/au/asls/land-surface/erosion-state-A"^^xsd:anyURI ;
  ui:isMemberOf  <erosion-state> ;
  rdfs:label "Active"@en ;
  skos:definition "one or both of the following conditions apply: evidence of sediment movement; sides and/or floors of erosion form are relatively bare of vegetation."@en ;
  skos:inScheme <> ;
  skos:notation "A" ;
  skos:prefLabel "Active"@en ;
  skos:topConceptOf <> ;
.
 <erosion-state-P>
  a skos:Concept ;
  dcterms:description "evidence of some active erosion and some evidence of stabilisation."@en ;
  dcterms:identifier "http://anzsoil.org/def/au/asls/land-surface/erosion-state-P"^^xsd:anyURI ;
  ui:isMemberOf  <erosion-state> ;
  rdfs:label "Partly stabilised"@en ;
  skos:definition "evidence of some active erosion and some evidence of stabilisation."@en ;
  skos:inScheme <> ;
  skos:notation "P" ;
  skos:prefLabel "Partly stabilised"@en ;
  skos:topConceptOf <> ;
.
 <erosion-state-S>
  a skos:Concept ;
  dcterms:description "one or both of the following conditions apply: no evidence of sediment movement; sides and/or floors of erosion form are revegetated."@en ;
  dcterms:identifier "http://anzsoil.org/def/au/asls/land-surface/erosion-state-S"^^xsd:anyURI ;
  ui:isMemberOf  <erosion-state> ;
  rdfs:label "Stabilised"@en ;
  skos:definition "one or both of the following conditions apply: no evidence of sediment movement; sides and/or floors of erosion form are revegetated."@en ;
  skos:inScheme <> ;
  skos:notation "S" ;
  skos:prefLabel "Stabilised"@en ;
  skos:topConceptOf <> ;
.
 <gilgai-microrelief>
  a skos:Collection ;
  dcterms:description "Gilgai is surface microrelief associated with soils containing shrink–swell clays. It does not include microrelief that apparently results from repeated freezing and thawing, solifluxion or faunal activity. Gilgai consist of mounds and depressions showing varying degrees of order, sometimes separated by a subplanar or slightly undulating surface."@en ;
  dcterms:identifier "http://anzsoil.org/def/au/asls/land-surface/gilgai-microrelief"^^xsd:anyURI ;
  ui:isMemberOf  <microrelief> ;
  rdfs:label "Gilgai microrelief"@en ;
  skos:definition "Gilgai is surface microrelief associated with soils containing shrink–swell clays. It does not include microrelief that apparently results from repeated freezing and thawing, solifluxion or faunal activity. Gilgai consist of mounds and depressions showing varying degrees of order, sometimes separated by a subplanar or slightly undulating surface."@en ;
  skos:member  <gilgai-microrelief-proportions> ;
  skos:member  <microrelief-A> ;
  skos:member  <microrelief-C> ;
  skos:member  <microrelief-G> ;
  skos:member  <microrelief-L> ;
  skos:member  <microrelief-M> ;
  skos:member  <microrelief-N> ;
  skos:prefLabel "Gilgai microrelief"@en ;
.
 <gilgai-microrelief-proportions>
  a skos:Collection ;
  a sosa:ObservableProperty ;
  dcterms:description "Give the proportions of gilgai components within the site, thus:"@en ;
  dcterms:identifier "http://anzsoil.org/def/au/asls/land-surface/gilgai-microrelief-proportions"^^xsd:anyURI ;
  ui:isMemberOf  <gilgai-microrelief> ;
  rdfs:label "Proportions of gilgai components "@en ;
  skos:definition "Give the proportions of gilgai components within the site, thus:"@en ;
  skos:member  <gilgai-microrelief-proportions-A> ;
  skos:member  <gilgai-microrelief-proportions-B> ;
  skos:member  <gilgai-microrelief-proportions-C> ;
  skos:member  <gilgai-microrelief-proportions-D> ;
  skos:prefLabel "Proportions of gilgai components "@en ;
.
 <gilgai-microrelief-proportions-A>
  a skos:Concept ;
  dcterms:description "Equal mounds and depressions; no shelf present."@en ;
  dcterms:identifier "http://anzsoil.org/def/au/asls/land-surface/gilgai-microrelief-proportions-A"^^xsd:anyURI ;
  ui:isMemberOf  <gilgai-microrelief-proportions> ;
  rdfs:label "Equal mounds and depressions; no shelf present"@en ;
  skos:definition "Equal mounds and depressions; no shelf present."@en ;
  skos:inScheme <> ;
  skos:notation "A" ;
  skos:prefLabel "Equal mounds and depressions; no shelf present"@en ;
  skos:topConceptOf <> ;
.
 <gilgai-microrelief-proportions-B>
  a skos:Concept ;
  dcterms:description "More mounds than depressions; no shelf present."@en ;
  dcterms:identifier "http://anzsoil.org/def/au/asls/land-surface/gilgai-microrelief-proportions-B"^^xsd:anyURI ;
  ui:isMemberOf  <gilgai-microrelief-proportions> ;
  rdfs:label "More mounds than depressions; no shelf present"@en ;
  skos:definition "More mounds than depressions; no shelf present."@en ;
  skos:inScheme <> ;
  skos:notation "B" ;
  skos:prefLabel "More mounds than depressions; no shelf present"@en ;
  skos:topConceptOf <> ;
.
 <gilgai-microrelief-proportions-C>
  a skos:Concept ;
  dcterms:description "Fewer mounds than depressions; no shelf present."@en ;
  dcterms:identifier "http://anzsoil.org/def/au/asls/land-surface/gilgai-microrelief-proportions-C"^^xsd:anyURI ;
  ui:isMemberOf  <gilgai-microrelief-proportions> ;
  rdfs:label "Fewer mounds than depressions; no shelf present"@en ;
  skos:definition "Fewer mounds than depressions; no shelf present."@en ;
  skos:inScheme <> ;
  skos:notation "C" ;
  skos:prefLabel "Fewer mounds than depressions; no shelf present"@en ;
  skos:topConceptOf <> ;
.
 <gilgai-microrelief-proportions-D>
  a skos:Concept ;
  dcterms:description "Mound, shelf and depressions; shelf forms prominent part of gilgai."@en ;
  dcterms:identifier "http://anzsoil.org/def/au/asls/land-surface/gilgai-microrelief-proportions-D"^^xsd:anyURI ;
  ui:isMemberOf  <gilgai-microrelief-proportions> ;
  rdfs:label "Mound, shelf and depressions; shelf forms prominent part of gilgai"@en ;
  skos:definition "Mound, shelf and depressions; shelf forms prominent part of gilgai."@en ;
  skos:inScheme <> ;
  skos:notation "D" ;
  skos:prefLabel "Mound, shelf and depressions; shelf forms prominent part of gilgai"@en ;
  skos:topConceptOf <> ;
.
 <hummocky-microrelief>
  a skos:Collection ;
  dcterms:description "Hummocky microrelief is not thought to be associated with the shrink–swell process involved in gilgai microrelief."@en ;
  dcterms:identifier "http://anzsoil.org/def/au/asls/land-surface/hummocky-microrelief"^^xsd:anyURI ;
  ui:isMemberOf  <microrelief> ;
  rdfs:label "Hummocky microrelief"@en ;
  skos:definition "Hummocky microrelief is not thought to be associated with the shrink–swell process involved in gilgai microrelief."@en ;
  skos:member  <microrelief-D> ;
  skos:member  <microrelief-W> ;
  skos:prefLabel "Hummocky microrelief"@en ;
.
 <inundation>
  a skos:Collection ;
  dcterms:description "Inundation includes flooding from over-bank flow, inundation from local runon and overland flow. Although the importance of this information is considerable, in most instances it cannot be assessed at each site. Some evidence may be available from past events, for example accumulation of debris in trees or on fences. Otherwise information is usually obtained from local enquiry."@en ;
  dcterms:identifier "http://anzsoil.org/def/au/asls/land-surface/inundation"^^xsd:anyURI ;
  ui:topMemberOf <> ;
  rdfs:label "Inundation"@en ;
  skos:definition "Inundation includes flooding from over-bank flow, inundation from local runon and overland flow. Although the importance of this information is considerable, in most instances it cannot be assessed at each site. Some evidence may be available from past events, for example accumulation of debris in trees or on fences. Otherwise information is usually obtained from local enquiry."@en ;
  skos:member  <inundation-depth> ;
  skos:member  <inundation-duration> ;
  skos:member  <inundation-frequency> ;
  skos:member  <inundation-runon-velocity> ;
  skos:prefLabel "Inundation"@en ;
.
 <inundation-depth>
  a skos:Collection ;
  a sosa:ObservableProperty ;
  dcterms:description "Give likely maximum depth of water in an inundation event (mm). "@en ;
  dcterms:identifier "http://anzsoil.org/def/au/asls/land-surface/inundation-depth"^^xsd:anyURI ;
  ui:isMemberOf  <inundation> ;
  rdfs:label "Depth of inundation (annual)"@en ;
  skos:definition "Give likely maximum depth of water in an inundation event (mm). "@en ;
  skos:member  <inundation-depth-1> ;
  skos:member  <inundation-depth-2> ;
  skos:member  <inundation-depth-3> ;
  skos:member  <inundation-depth-4> ;
  skos:member  <inundation-depth-5> ;
  skos:prefLabel "Depth of inundation (annual)"@en ;
.
 <inundation-depth-1>
  a skos:Concept ;
  dcterms:description "<50 mm"@en ;
  dcterms:identifier "http://anzsoil.org/def/au/asls/land-surface/inundation-depth-1"^^xsd:anyURI ;
  ui:isMemberOf  <inundation-depth> ;
  rdfs:label "Inundation depth <50 mm"@en ;
  skos:definition "<50 mm"@en ;
  skos:inScheme <> ;
  skos:notation "1" ;
  skos:prefLabel "Inundation depth <50 mm"@en ;
  skos:topConceptOf <> ;
.
 <inundation-depth-2>
  a skos:Concept ;
  dcterms:description "50-100 mm"@en ;
  dcterms:identifier "http://anzsoil.org/def/au/asls/land-surface/inundation-depth-2"^^xsd:anyURI ;
  ui:isMemberOf  <inundation-depth> ;
  rdfs:label "Inundation 50-100 mm"@en ;
  skos:definition "depth 50-100 mm"@en ;
  skos:inScheme <> ;
  skos:notation "2" ;
  skos:prefLabel "Inundation depth 50-100 mm"@en ;
  skos:topConceptOf <> ;
.
 <inundation-depth-3>
  a skos:Concept ;
  dcterms:description "100-300 mm"@en ;
  dcterms:identifier "http://anzsoil.org/def/au/asls/land-surface/inundation-depth-3"^^xsd:anyURI ;
  ui:isMemberOf  <inundation-depth> ;
  rdfs:label "Inundation depth 100-300 mm"@en ;
  skos:definition "100-300 mm"@en ;
  skos:inScheme <> ;
  skos:notation "3" ;
  skos:prefLabel "Inundation depth 100-300 mm"@en ;
  skos:topConceptOf <> ;
.
 <inundation-depth-4>
  a skos:Concept ;
  dcterms:description "300-1000 mm"@en ;
  dcterms:identifier "http://anzsoil.org/def/au/asls/land-surface/inundation-depth-4"^^xsd:anyURI ;
  ui:isMemberOf  <inundation-depth> ;
  rdfs:label "Inundation depth 300-1000 mm"@en ;
  skos:definition "300-1000 mm"@en ;
  skos:inScheme <> ;
  skos:notation "4" ;
  skos:prefLabel "Inundation depth 300-1000 mm"@en ;
  skos:topConceptOf <> ;
.
 <inundation-depth-5>
  a skos:Concept ;
  dcterms:description ">1000 mm"@en ;
  dcterms:identifier "http://anzsoil.org/def/au/asls/land-surface/inundation-depth-5"^^xsd:anyURI ;
  ui:isMemberOf  <inundation-depth> ;
  rdfs:label "Inundation depth >1000 mm"@en ;
  skos:definition ">1000 mm"@en ;
  skos:inScheme <> ;
  skos:notation "5" ;
  skos:prefLabel "Inundation depth >1000 mm"@en ;
  skos:topConceptOf <> ;
.
 <inundation-duration>
  a skos:Collection ;
  a sosa:ObservableProperty ;
  dcterms:description "Give likely duration of an inundation event."@en ;
  dcterms:identifier "http://anzsoil.org/def/au/asls/land-surface/inundation-duration"^^xsd:anyURI ;
  ui:isMemberOf  <inundation> ;
  rdfs:label "Duration (annual) of inundation"@en ;
  skos:definition "Give likely duration of an inundation event."@en ;
  skos:member  <inundation-duration-1> ;
  skos:member  <inundation-duration-2> ;
  skos:member  <inundation-duration-3> ;
  skos:member  <inundation-duration-4> ;
  skos:prefLabel "Duration (annual) of inundation"@en ;
.
 <inundation-duration-1>
  a skos:Concept ;
  dcterms:description "Less than 1 day"@en ;
  dcterms:identifier "http://anzsoil.org/def/au/asls/land-surface/inundation-duration-1"^^xsd:anyURI ;
  ui:isMemberOf  <inundation-duration> ;
  rdfs:label "Less than 1 day"@en ;
  skos:definition "Less than 1 day"@en ;
  skos:inScheme <> ;
  skos:notation "1" ;
  skos:prefLabel "Less than 1 day"@en ;
  skos:topConceptOf <> ;
.
 <inundation-duration-2>
  a skos:Concept ;
  dcterms:description "Between 1 and 20 days"@en ;
  dcterms:identifier "http://anzsoil.org/def/au/asls/land-surface/inundation-duration-2"^^xsd:anyURI ;
  ui:isMemberOf  <inundation-duration> ;
  rdfs:label "Between 1 and 20 days"@en ;
  skos:definition "Between 1 and 20 days"@en ;
  skos:inScheme <> ;
  skos:notation "2" ;
  skos:prefLabel "Between 1 and 20 days"@en ;
  skos:topConceptOf <> ;
.
 <inundation-duration-3>
  a skos:Concept ;
  dcterms:description "Between 20 and 120 days"@en ;
  dcterms:identifier "http://anzsoil.org/def/au/asls/land-surface/inundation-duration-3"^^xsd:anyURI ;
  ui:isMemberOf  <inundation-duration> ;
  rdfs:label "Between 20 and 120 days"@en ;
  skos:definition "Between 20 and 120 days"@en ;
  skos:inScheme <> ;
  skos:notation "3" ;
  skos:prefLabel "Between 20 and 120 days"@en ;
  skos:topConceptOf <> ;
.
 <inundation-duration-4>
  a skos:Concept ;
  dcterms:description "More than 120 days"@en ;
  dcterms:identifier "http://anzsoil.org/def/au/asls/land-surface/inundation-duration-4"^^xsd:anyURI ;
  ui:isMemberOf  <inundation-duration> ;
  rdfs:label "More than 120 days"@en ;
  skos:definition "More than 120 days"@en ;
  skos:inScheme <> ;
  skos:notation "4" ;
  skos:prefLabel "More than 120 days"@en ;
  skos:topConceptOf <> ;
.
 <inundation-frequency>
  a skos:Collection ;
  a sosa:ObservableProperty ;
  dcterms:description "Give long-term average of inundation. Among alluvial plains, flood plains typically fall in categories 4 and 3."@en ;
  dcterms:identifier "http://anzsoil.org/def/au/asls/land-surface/inundation-frequency"^^xsd:anyURI ;
  ui:isMemberOf  <inundation> ;
  rdfs:label "Frequency of inundation"@en ;
  skos:definition "Give long-term average of inundation. Among alluvial plains, flood plains typically fall in categories 4 and 3."@en ;
  skos:member  <inundation-frequency-0> ;
  skos:member  <inundation-frequency-1> ;
  skos:member  <inundation-frequency-2> ;
  skos:member  <inundation-frequency-3> ;
  skos:member  <inundation-frequency-4> ;
  skos:member  <inundation-frequency-5> ;
  skos:prefLabel "Frequency of inundation"@en ;
.
 <inundation-frequency-0>
  a skos:Concept ;
  dcterms:description "No inundation."@en ;
  dcterms:identifier "http://anzsoil.org/def/au/asls/land-surface/inundation-frequency-0"^^xsd:anyURI ;
  ui:isMemberOf  <inundation-frequency> ;
  rdfs:label "No inundation"@en ;
  skos:definition "No inundation."@en ;
  skos:inScheme <> ;
  skos:notation "0" ;
  skos:prefLabel "No inundation"@en ;
  skos:topConceptOf <> ;
.
 <inundation-frequency-1>
  a skos:Concept ;
  dcterms:description "Less than one occurrence per 100 years."@en ;
  dcterms:identifier "http://anzsoil.org/def/au/asls/land-surface/inundation-frequency-1"^^xsd:anyURI ;
  ui:isMemberOf  <inundation-frequency> ;
  rdfs:label "Less than one occurrence per 100 years"@en ;
  skos:definition "Less than one occurrence per 100 years. "@en ;
  skos:inScheme <> ;
  skos:notation "1" ;
  skos:prefLabel "Less than one occurrence per 100 years"@en ;
  skos:topConceptOf <> ;
.
 <inundation-frequency-2>
  a skos:Concept ;
  dcterms:description "One occurrence in between 50 and 100 years."@en ;
  dcterms:identifier "http://anzsoil.org/def/au/asls/land-surface/inundation-frequency-2"^^xsd:anyURI ;
  ui:isMemberOf  <inundation-frequency> ;
  rdfs:label "One occurrence in between 50 and 100 years"@en ;
  skos:definition "One occurrence in between 50 and 100 years. "@en ;
  skos:inScheme <> ;
  skos:notation "2" ;
  skos:prefLabel "One occurrence in between 50 and 100 years"@en ;
  skos:topConceptOf <> ;
.
 <inundation-frequency-3>
  a skos:Concept ;
  dcterms:description "One occurrence in between 10 and 50 years."@en ;
  dcterms:identifier "http://anzsoil.org/def/au/asls/land-surface/inundation-frequency-3"^^xsd:anyURI ;
  ui:isMemberOf  <inundation-frequency> ;
  rdfs:label "One occurrence in between 10 and 50 years"@en ;
  skos:definition "One occurrence in between 10 and 50 years. "@en ;
  skos:inScheme <> ;
  skos:notation "3" ;
  skos:prefLabel "One occurrence in between 10 and 50 years"@en ;
  skos:topConceptOf <> ;
.
 <inundation-frequency-4>
  a skos:Concept ;
  dcterms:description "One occurrence in between 1 and 10 years."@en ;
  dcterms:identifier "http://anzsoil.org/def/au/asls/land-surface/inundation-frequency-4"^^xsd:anyURI ;
  ui:isMemberOf  <inundation-frequency> ;
  rdfs:label "One occurrence in between 1 and 10 years"@en ;
  skos:definition "One occurrence in between 1 and 10 years. "@en ;
  skos:inScheme <> ;
  skos:notation "4" ;
  skos:prefLabel "One occurrence in between 1 and 10 years"@en ;
  skos:topConceptOf <> ;
.
 <inundation-frequency-5>
  a skos:Concept ;
  dcterms:description "More than one occurrence per year."@en ;
  dcterms:identifier "http://anzsoil.org/def/au/asls/land-surface/inundation-frequency-5"^^xsd:anyURI ;
  ui:isMemberOf  <inundation-frequency> ;
  rdfs:label "More than one occurrence per year"@en ;
  skos:definition "More than one occurrence per year. "@en ;
  skos:inScheme <> ;
  skos:notation "5" ;
  skos:prefLabel "More than one occurrence per year"@en ;
  skos:topConceptOf <> ;
.
 <inundation-runon-velocity>
  a skos:Collection ;
  a sosa:ObservableProperty ;
  dcterms:description "As a guide, the surface velocity in a river is typically 1–2 m/s. "@en ;
  dcterms:identifier "http://anzsoil.org/def/au/asls/land-surface/inundation-runon-velocity"^^xsd:anyURI ;
  ui:isMemberOf  <inundation> ;
  rdfs:label "Runon velocity of inundation"@en ;
  skos:definition "As a guide, the surface velocity in a river is typically 1–2 m/s. "@en ;
  skos:member  <inundation-runon-velocity-H> ;
  skos:member  <inundation-runon-velocity-L> ;
  skos:prefLabel "Runon velocity of inundation"@en ;
.
 <inundation-runon-velocity-H>
  a skos:Concept ;
  dcterms:description "High velocity >300 mm/s"@en ;
  dcterms:identifier "http://anzsoil.org/def/au/asls/land-surface/inundation-runon-velocity-H"^^xsd:anyURI ;
  ui:isMemberOf  <inundation-frequency> ;
  rdfs:label "High velocity >300 mm/s"@en ;
  skos:definition "High velocity >300 mm/s"@en ;
  skos:inScheme <> ;
  skos:notation "H" ;
  skos:prefLabel "High velocity >300 mm/s"@en ;
  skos:topConceptOf <> ;
.
 <inundation-runon-velocity-L>
  a skos:Concept ;
  dcterms:description "Low velocity <300 mm/s"@en ;
  dcterms:identifier "http://anzsoil.org/def/au/asls/land-surface/inundation-runon-velocity-L"^^xsd:anyURI ;
  ui:isMemberOf  <inundation-frequency> ;
  rdfs:label "Low velocity <300 mm/s"@en ;
  skos:definition "Low velocity <300 mm/s"@en ;
  skos:inScheme <> ;
  skos:notation "L" ;
  skos:prefLabel "Low velocity <300 mm/s"@en ;
  skos:topConceptOf <> ;
.
 <lithology-CC>
  a skos:Concept ;
  dcterms:description "Charcoal"@en ;
  dcterms:identifier "http://anzsoil.org/def/au/asls/land-surface/lithology-CC"^^xsd:anyURI ;
  ui:isMemberOf  <coarse-fragments-lithology> ;
  rdfs:comment "C_LITHOLOGY" ;
  rdfs:label "Charcoal"@en ;
  skos:definition "Charcoal"@en ;
  skos:inScheme <> ;
  skos:notation "CC" ;
  skos:prefLabel "Charcoal"@en ;
  skos:topConceptOf <> ;
.
 <lithology-IS>
  a skos:Concept ;
  dcterms:description "Ironstone (where not considered of pedogenic origin)"@en ;
  dcterms:identifier "http://anzsoil.org/def/au/asls/land-surface/lithology-IS"^^xsd:anyURI ;
  ui:isMemberOf  <coarse-fragments-lithology> ;
  rdfs:comment "C_LITHOLOGY" ;
  rdfs:label "Ironstone"@en ;
  skos:definition "Ironstone (where not considered of pedogenic origin)"@en ;
  skos:inScheme <> ;
  skos:notation "IS" ;
  skos:prefLabel "Ironstone"@en ;
  skos:topConceptOf <> ;
.
 <lithology-OT>
  a skos:Concept ;
  dcterms:description "Other"@en ;
  dcterms:identifier "http://anzsoil.org/def/au/asls/land-surface/lithology-OT"^^xsd:anyURI ;
  ui:isMemberOf  <coarse-fragments-lithology> ;
  rdfs:comment "C_LITHOLOGY" ;
  rdfs:label "Other"@en ;
  skos:definition "Other"@en ;
  skos:inScheme <> ;
  skos:notation "OT" ;
  skos:prefLabel "Other"@en ;
  skos:topConceptOf <> ;
.
 <lithology-OW>
  a skos:Concept ;
  dcterms:description "Opalised wood"@en ;
  dcterms:identifier "http://anzsoil.org/def/au/asls/land-surface/lithology-OW"^^xsd:anyURI ;
  ui:isMemberOf  <coarse-fragments-lithology> ;
  rdfs:comment "C_LITHOLOGY" ;
  rdfs:label "Opalised wood"@en ;
  skos:definition "Opalised wood"@en ;
  skos:inScheme <> ;
  skos:notation "OW" ;
  skos:prefLabel "Opalised wood"@en ;
  skos:topConceptOf <> ;
.
 <lithology-PU>
  a skos:Concept ;
  dcterms:description "Pumice"@en ;
  dcterms:identifier "http://anzsoil.org/def/au/asls/land-surface/lithology-PU"^^xsd:anyURI ;
  ui:isMemberOf  <coarse-fragments-lithology> ;
  rdfs:comment "C_LITHOLOGY" ;
  rdfs:label "Pumice"@en ;
  skos:definition "Pumice"@en ;
  skos:inScheme <> ;
  skos:notation "PU" ;
  skos:prefLabel "Pumice"@en ;
  skos:topConceptOf <> ;
.
 <lithology-SS>
  a skos:Concept ;
  dcterms:description "Shells"@en ;
  dcterms:identifier "http://anzsoil.org/def/au/asls/land-surface/lithology-SS"^^xsd:anyURI ;
  ui:isMemberOf  <coarse-fragments-lithology> ;
  rdfs:comment "C_LITHOLOGY" ;
  rdfs:label "Shells"@en ;
  skos:definition "Shells"@en ;
  skos:inScheme <> ;
  skos:notation "SS" ;
  skos:prefLabel "Shells"@en ;
  skos:topConceptOf <> ;
.
 <microrelief>
  a skos:Collection ;
  a sosa:ObservableProperty ;
  dcterms:description "Microrelief refers to relief up to a few metres about the plane of the land surface. It includes gilgai, hummocky, biotic and other microrelief."@en ;
  dcterms:identifier "http://anzsoil.org/def/au/asls/land-surface/microrelief"^^xsd:anyURI ;
  ui:topMemberOf <> ;
  rdfs:label "Microrelief"@en ;
  skos:definition "Microrelief refers to relief up to a few metres about the plane of the land surface. It includes gilgai, hummocky, biotic and other microrelief."@en ;
  skos:member  <biotic-microrelief> ;
  skos:member  <gilgai-microrelief> ;
  skos:member  <hummocky-microrelief> ;
  skos:member  <microrelief-Z> ;
  skos:member  <microrelief-component-sampled> ;
  skos:member  <microrelief-horizontal-interval> ;
  skos:member  <microrelief-vertical-interval> ;
  skos:member  <other-microrelief-O> ;
  skos:prefLabel "Microrelief"@en ;
.
 <microrelief-A>
  a skos:Concept ;
  dcterms:description "discontinuous, elongate mounds and/or elongate depressions more or less at right angles to the contour. Usually in sloping lands, commonly between linear gilgai on lower slopes and plains."@en ;
  dcterms:identifier "http://anzsoil.org/def/au/asls/land-surface/microrelief-A"^^xsd:anyURI ;
  ui:isMemberOf  <gilgai-microrelief> ;
  rdfs:label "Lattice gilgai"@en ;
  skos:definition "discontinuous, elongate mounds and/or elongate depressions more or less at right angles to the contour. Usually in sloping lands, commonly between linear gilgai on lower slopes and plains."@en ;
  skos:inScheme <> ;
  skos:notation "A" ;
  skos:prefLabel "Lattice gilgai"@en ;
  skos:topConceptOf <> ;
.
 <microrelief-C>
  a skos:Concept ;
  dcterms:description "irregularly distributed, small depressions and mounds separated by a more or less continuous shelf. Vertical interval usually less than 0.3 m. Horizontal interval usually 3–20 m, surface almost level."@en ;
  dcterms:identifier "http://anzsoil.org/def/au/asls/land-surface/microrelief-C"^^xsd:anyURI ;
  ui:isMemberOf  <gilgai-microrelief> ;
  rdfs:comment "Vertical interval usually < 0.3 m and horizontal interval 3 - 20m"@en ;
  rdfs:label "Crabhole gilgai"@en ;
  skos:definition "irregularly distributed, small depressions and mounds separated by a more or less continuous shelf. Vertical interval usually less than 0.3 m. Horizontal interval usually 3–20 m, surface almost level."@en ;
  skos:inScheme <> ;
  skos:notation "C" ;
  skos:prefLabel "Crabhole gilgai"@en ;
  skos:topConceptOf <> ;
.
 <microrelief-D>
  a skos:Concept ;
  dcterms:description "small hummocks rising above a planar surface. They vary from rounded, both planar and vertically, to flat-topped, relatively steep-sided and elongate. They are usually closely and regularly spaced, ranging from 0.06 to 0.6 m in both vertical and horizontal dimensions. They are common in northern Australia on soils with impeded internal drainage and in areas of short seasonal ponding. Many observers consider them to be formed by biological activity."@en ;
  dcterms:identifier "http://anzsoil.org/def/au/asls/land-surface/microrelief-D"^^xsd:anyURI ;
  ui:isMemberOf  <hummocky-microrelief> ;
  rdfs:label "Debil-debil"@en ;
  skos:definition "small hummocks rising above a planar surface. They vary from rounded, both planar and vertically, to flat-topped, relatively steep-sided and elongate. They are usually closely and regularly spaced, ranging from 0.06 to 0.6 m in both vertical and horizontal dimensions. They are common in northern Australia on soils with impeded internal drainage and in areas of short seasonal ponding. Many observers consider them to be formed by biological activity."@en ;
  skos:inScheme <> ;
  skos:notation "D" ;
  skos:prefLabel "Debil-debil"@en ;
  skos:topConceptOf <> ;
.
 <microrelief-G>
  a skos:Concept ;
  dcterms:description "irregularly distributed, large depressions, usually greater than 3 m in diameter or greatest dimension, subcircular or irregular and varying from closely spaced in a network of elongate mounds to isolated depressions set in an undulating shelf with occasional small mounds. Some depressions may also contain sinkholes of gilgai usually greater than 0.3 m; horizontal interval usually 5–6 m; surface almost level."@en ;
  dcterms:identifier "http://anzsoil.org/def/au/asls/land-surface/microrelief-G"^^xsd:anyURI ;
  ui:isMemberOf  <gilgai-microrelief> ;
  rdfs:label "Contour gilgai"@en ;
  skos:definition "irregularly distributed, large depressions, usually greater than 3 m in diameter or greatest dimension, subcircular or irregular and varying from closely spaced in a network of elongate mounds to isolated depressions set in an undulating shelf with occasional small mounds. Some depressions may also contain sinkholes of gilgai usually greater than 0.3 m; horizontal interval usually 5–6 m; surface almost level."@en ;
  skos:inScheme <> ;
  skos:notation "G" ;
  skos:prefLabel "Contour gilgai"@en ;
  skos:topConceptOf <> ;
.
 <microrelief-H>
  a skos:Concept ;
  dcterms:description "Depression associated with water flowing from rock or soil without the agency of man."@en ;
  dcterms:identifier "http://anzsoil.org/def/au/asls/land-surface/microrelief-H"^^xsd:anyURI ;
  ui:isMemberOf  <other-microrelief-O> ;
  rdfs:label "Spring hollow"@en ;
  skos:definition "Depression associated with water flowing from rock or soil without the agency of man."@en ;
  skos:inScheme <> ;
  skos:notation "H" ;
  skos:prefLabel "Spring hollow"@en ;
  skos:topConceptOf <> ;
.
 <microrelief-I>
  a skos:Concept ;
  dcterms:description "closed depression with vertical or funnel-shaped sides."@en ;
  dcterms:identifier "http://anzsoil.org/def/au/asls/land-surface/microrelief-I"^^xsd:anyURI ;
  ui:isMemberOf  <other-microrelief-O> ;
  rdfs:label "Sinkhole"@en ;
  skos:definition "closed depression with vertical or funnel-shaped sides."@en ;
  skos:inScheme <> ;
  skos:notation "I" ;
  skos:prefLabel "Sinkhole"@en ;
  skos:topConceptOf <> ;
.
 <microrelief-K>
  a skos:Concept ;
  dcterms:description "depressions in limestone country."@en ;
  dcterms:identifier "http://anzsoil.org/def/au/asls/land-surface/microrelief-K"^^xsd:anyURI ;
  ui:isMemberOf  <other-microrelief-O> ;
  rdfs:label "Karst microrelief"@en ;
  skos:definition "depressions in limestone country."@en ;
  skos:inScheme <> ;
  skos:notation "K" ;
  skos:prefLabel "Karst microrelief"@en ;
  skos:topConceptOf <> ;
.
 <microrelief-L>
  a skos:Concept ;
  dcterms:description "long, narrow, parallel, elongate mounds and broader elongate depressions more or less at right angles to the contour. Usually in sloping lands. Vertical interval usually less than 0.3 m, horizontal interval usually 5–8 m."@en ;
  dcterms:identifier "http://anzsoil.org/def/au/asls/land-surface/microrelief-L"^^xsd:anyURI ;
  ui:isMemberOf  <gilgai-microrelief> ;
  rdfs:comment "Vertical interval usually < 0.3 m and horizontal interval 5 - 8 m"@en ;
  rdfs:label "Linear gilgai"@en ;
  skos:definition "long, narrow, parallel, elongate mounds and broader elongate depressions more or less at right angles to the contour. Usually in sloping lands. Vertical interval usually less than 0.3 m, horizontal interval usually 5–8 m."@en ;
  skos:inScheme <> ;
  skos:notation "L" ;
  skos:prefLabel "Linear gilgai"@en ;
  skos:topConceptOf <> ;
.
 <microrelief-M>
  a skos:Concept ;
  dcterms:description "irregularly distributed, large depressions, usually greater than 3 m in diameter or greatest dimension, subcircular or irregular and varying from closely spaced in a network of elongate mounds to isolated depressions set in an undulating shelf with occasional small mounds. Some depressions may also contain sinkholes of gilgai usually greater than 0.3 m; horizontal interval usually 5–6 m; surface almost level."@en ;
  dcterms:identifier "http://anzsoil.org/def/au/asls/land-surface/microrelief-M"^^xsd:anyURI ;
  ui:isMemberOf  <gilgai-microrelief> ;
  rdfs:label "Melonhole gilgai"@en ;
  skos:definition "irregularly distributed, large depressions, usually greater than 3 m in diameter or greatest dimension, subcircular or irregular and varying from closely spaced in a network of elongate mounds to isolated depressions set in an undulating shelf with occasional small mounds. Some depressions may also contain sinkholes of gilgai usually greater than 0.3 m; horizontal interval usually 5–6 m; surface almost level."@en ;
  skos:inScheme <> ;
  skos:notation "M" ;
  skos:prefLabel "Melonhole gilgai"@en ;
  skos:topConceptOf <> ;
.
 <microrelief-N>
  a skos:Concept ;
  dcterms:description "irregularly distributed, small mounds and subcircular depressions varying in size and spacing. Vertical interval usually less than 0.3 m, horizontal interval usually 3–10 m, surface almost level."@en ;
  dcterms:identifier "http://anzsoil.org/def/au/asls/land-surface/microrelief-N"^^xsd:anyURI ;
  ui:isMemberOf  <gilgai-microrelief> ;
  rdfs:comment "Vertical interval usually < 0.3 m and horizontal interval 3 - 10m"@en ;
  rdfs:label "Normal gilgai"@en ;
  skos:definition "irregularly distributed, small mounds and subcircular depressions varying in size and spacing. Vertical interval usually less than 0.3 m, horizontal interval usually 3–10 m, surface almost level."@en ;
  skos:inScheme <> ;
  skos:notation "N" ;
  skos:prefLabel "Normal gilgai"@en ;
  skos:topConceptOf <> ;
.
 <microrelief-P>
  a skos:Concept ;
  dcterms:description "Mound associated with water flowing from rock or soil without the agency of man."@en ;
  dcterms:identifier "http://anzsoil.org/def/au/asls/land-surface/microrelief-P"^^xsd:anyURI ;
  ui:isMemberOf  <other-microrelief-O> ;
  rdfs:label "Spring mound"@en ;
  skos:definition "Mound associated with water flowing from rock or soil without the agency of man."@en ;
  skos:inScheme <> ;
  skos:notation "P" ;
  skos:prefLabel "Spring mound"@en ;
  skos:topConceptOf <> ;
.
 <microrelief-R>
  a skos:Concept ;
  dcterms:description "small terraces on slopes resulting either from soil creep or trampling by hoofed animals."@en ;
  dcterms:identifier "http://anzsoil.org/def/au/asls/land-surface/microrelief-R"^^xsd:anyURI ;
  ui:isMemberOf  <other-microrelief-O> ;
  rdfs:label "Terracettes"@en ;
  skos:definition "small terraces on slopes resulting either from soil creep or trampling by hoofed animals."@en ;
  skos:inScheme <> ;
  skos:notation "R" ;
  skos:prefLabel "Terracettes"@en ;
  skos:topConceptOf <> ;
.
 <microrelief-S>
  a skos:Concept ;
  dcterms:description "hummocky microrelief on the surface of landslides, slumps, earth flows, debris avalanches."@en ;
  dcterms:identifier "http://anzsoil.org/def/au/asls/land-surface/microrelief-S"^^xsd:anyURI ;
  ui:isMemberOf  <other-microrelief-O> ;
  rdfs:label "Mass movement microrelief"@en ;
  skos:definition "hummocky microrelief on the surface of landslides, slumps, earth flows, debris avalanches."@en ;
  skos:inScheme <> ;
  skos:notation "S" ;
  skos:prefLabel "Mass movement microrelief"@en ;
  skos:topConceptOf <> ;
.
 <microrelief-T>
  a skos:Concept ;
  dcterms:description "trenches typically 0.2 m deep and 0.6 m wide, with near vertical walls, alternating with flat-crested ridges about 1.3 m wide, which extend along the contour for several metres or tens of metres. Contour trenches are known in areas in south-eastern Australia above 350 m altitude with a high effective rainfall, where they are associated with a grassland or heathland vegetation on undulating rises (compare with McElroy 1952)."@en ;
  dcterms:identifier "http://anzsoil.org/def/au/asls/land-surface/microrelief-T"^^xsd:anyURI ;
  ui:isMemberOf  <other-microrelief-O> ;
  rdfs:label "Contour trench"@en ;
  skos:definition "trenches typically 0.2 m deep and 0.6 m wide, with near vertical walls, alternating with flat-crested ridges about 1.3 m wide, which extend along the contour for several metres or tens of metres. Contour trenches are known in areas in south-eastern Australia above 350 m altitude with a high effective rainfall, where they are associated with a grassland or heathland vegetation on undulating rises (compare with McElroy 1952)."@en ;
  skos:inScheme <> ;
  skos:notation "T" ;
  skos:prefLabel "Contour trench"@en ;
  skos:topConceptOf <> ;
.
 <microrelief-U>
  a skos:Concept ;
  dcterms:description "undifferentiated, irregularly distributed or isolated mounds and/or depressions set in a planar surface."@en ;
  dcterms:identifier "http://anzsoil.org/def/au/asls/land-surface/microrelief-U"^^xsd:anyURI ;
  ui:isMemberOf  <other-microrelief-O> ;
  rdfs:label "Mound/depression microrelief"@en ;
  skos:definition "undifferentiated, irregularly distributed or isolated mounds and/or depressions set in a planar surface."@en ;
  skos:inScheme <> ;
  skos:notation "U" ;
  skos:prefLabel "Mound/depression microrelief"@en ;
  skos:topConceptOf <> ;
.
 <microrelief-W>
  a skos:Concept ;
  dcterms:description "steep-sided hummocks rising above a flat surface. Hummocks are frequently occupied by trees or shrubs while the lower surface may be vegetation free or occupied by sedges or reeds. They are subject to prolonged seasonal flooding."@en ;
  dcterms:identifier "http://anzsoil.org/def/au/asls/land-surface/microrelief-W"^^xsd:anyURI ;
  ui:isMemberOf  <hummocky-microrelief> ;
  rdfs:label "Swamp hummock"@en ;
  skos:definition "steep-sided hummocks rising above a flat surface. Hummocks are frequently occupied by trees or shrubs while the lower surface may be vegetation free or occupied by sedges or reeds. They are subject to prolonged seasonal flooding. "@en ;
  skos:inScheme <> ;
  skos:notation "W" ;
  skos:prefLabel "Swamp hummock"@en ;
  skos:topConceptOf <> ;
.
 <microrelief-Z>
  a skos:Concept ;
  dcterms:description "Zero or no microrelief"@en ;
  dcterms:identifier "http://anzsoil.org/def/au/asls/land-surface/microrelief-Z"^^xsd:anyURI ;
  ui:isMemberOf  <microrelief> ;
  rdfs:label "Zero or no microrelief"@en ;
  skos:definition "Zero or no microrelief"@en ;
  skos:inScheme <> ;
  skos:notation "Z" ;
  skos:prefLabel "Zero or no microrelief"@en ;
  skos:topConceptOf <> ;
.
 <microrelief-component-D>
  a skos:Concept ;
  dcterms:description "concave; occurs as closed form."@en ;
  dcterms:identifier "http://anzsoil.org/def/au/asls/land-surface/microrelief-component-D"^^xsd:anyURI ;
  ui:isMemberOf  <microrelief-component-sampled> ;
  rdfs:label "Depression"@en ;
  skos:definition "concave; occurs as closed form."@en ;
  skos:inScheme <> ;
  skos:notation "D" ;
  skos:prefLabel "Depression"@en ;
  skos:topConceptOf <> ;
.
 <microrelief-component-E>
  a skos:Concept ;
  dcterms:description "convex; long axis* more than 3 times the shorter axis."@en ;
  dcterms:identifier "http://anzsoil.org/def/au/asls/land-surface/microrelief-component-E"^^xsd:anyURI ;
  ui:isMemberOf  <microrelief-component-sampled> ;
  rdfs:label "Elongate mound"@en ;
  skos:definition "convex; long axis* more than 3 times the shorter axis."@en ;
  skos:inScheme <> ;
  skos:notation "E" ;
  skos:prefLabel "Elongate mound"@en ;
  skos:topConceptOf <> ;
.
 <microrelief-component-F>
  a skos:Concept ;
  dcterms:description "surface in which hummocks, mounds, depressions or sinkholes are set."@en ;
  dcterms:identifier "http://anzsoil.org/def/au/asls/land-surface/microrelief-component-F"^^xsd:anyURI ;
  ui:isMemberOf  <microrelief-component-sampled> ;
  rdfs:label "Flat"@en ;
  skos:definition "surface in which hummocks, mounds, depressions or sinkholes are set."@en ;
  skos:inScheme <> ;
  skos:notation "F" ;
  skos:prefLabel "Flat"@en ;
  skos:topConceptOf <> ;
.
 <microrelief-component-K>
  a skos:Concept ;
  dcterms:description "rises above a flat or planar surface. Sides vary from rounded to near vertical and tops from rounded to flat."@en ;
  dcterms:identifier "http://anzsoil.org/def/au/asls/land-surface/microrelief-component-K"^^xsd:anyURI ;
  ui:isMemberOf  <microrelief-component-sampled> ;
  rdfs:label "Hummock"@en ;
  skos:definition "rises above a flat or planar surface. Sides vary from rounded to near vertical and tops from rounded to flat."@en ;
  skos:inScheme <> ;
  skos:notation "K" ;
  skos:prefLabel "Hummock"@en ;
  skos:topConceptOf <> ;
.
 <microrelief-component-L>
  a skos:Concept ;
  dcterms:description "concave; occurs as open-ended form."@en ;
  dcterms:identifier "http://anzsoil.org/def/au/asls/land-surface/microrelief-component-L"^^xsd:anyURI ;
  ui:isMemberOf  <microrelief-component-sampled> ;
  rdfs:label "Elongate depression"@en ;
  skos:definition "concave; occurs as open-ended form."@en ;
  skos:inScheme <> ;
  skos:notation "L" ;
  skos:prefLabel "Elongate depression"@en ;
  skos:topConceptOf <> ;
.
 <microrelief-component-M>
  a skos:Concept ;
  dcterms:description "convex; long axis* not more than 3 times the shorter axis."@en ;
  dcterms:identifier "http://anzsoil.org/def/au/asls/land-surface/microrelief-component-M"^^xsd:anyURI ;
  ui:isMemberOf  <microrelief-component-sampled> ;
  rdfs:label "Mound"@en ;
  skos:definition "convex; long axis* not more than 3 times the shorter axis."@en ;
  skos:inScheme <> ;
  skos:notation "M" ;
  skos:prefLabel "Mound"@en ;
  skos:topConceptOf <> ;
.
 <microrelief-component-S>
  a skos:Concept ;
  dcterms:description "more or less planar; occurs between mounds and depressions."@en ;
  dcterms:identifier "http://anzsoil.org/def/au/asls/land-surface/microrelief-component-S"^^xsd:anyURI ;
  ui:isMemberOf  <microrelief-component-sampled> ;
  rdfs:label "Shelf"@en ;
  skos:definition "more or less planar; occurs between mounds and depressions."@en ;
  skos:inScheme <> ;
  skos:notation "S" ;
  skos:prefLabel "Shelf"@en ;
  skos:topConceptOf <> ;
.
 <microrelief-component-sampled>
  a skos:Collection ;
  a sosa:ObservableProperty ;
  dcterms:description "Give the component of the microrelief in which the described soil profile is located."@en ;
  dcterms:identifier "http://anzsoil.org/def/au/asls/land-surface/microrelief-component-sampled"^^xsd:anyURI ;
  ui:isMemberOf  <microrelief> ;
  rdfs:label "Component of microrelief sampled"@en ;
  skos:definition "Give the component of the microrelief in which the described soil profile is located."@en ;
  skos:member  <microrelief-component-D> ;
  skos:member  <microrelief-component-E> ;
  skos:member  <microrelief-component-F> ;
  skos:member  <microrelief-component-K> ;
  skos:member  <microrelief-component-L> ;
  skos:member  <microrelief-component-M> ;
  skos:member  <microrelief-component-S> ;
  skos:prefLabel "Component of microrelief sampled"@en ;
.
 <microrelief-horizontal-interval>
  a skos:Concept ;
  a sosa:ObservableProperty ;
  dcterms:description "Give horizontal distance, in metres, between crests of mounds or tops of hummocks."@en ;
  dcterms:identifier "http://anzsoil.org/def/au/asls/land-surface/microrelief-horizontal-interval"^^xsd:anyURI ;
  ui:isMemberOf  <microrelief> ;
  rdfs:label "Horizontal interval"@en ;
  skos:definition "Give horizontal distance, in metres, between crests of mounds or tops of hummocks."@en ;
  skos:inScheme <> ;
  skos:prefLabel "Horizontal interval"@en ;
  skos:topConceptOf <> ;
.
 <microrelief-vertical-interval>
  a skos:Concept ;
  dcterms:description "Give vertical distance, in metres, between base of depression or flat and horizontal line joining crests of mounds or hummocks."@en ;
  dcterms:identifier "http://anzsoil.org/def/au/asls/land-surface/microrelief-vertical-interval"^^xsd:anyURI ;
  ui:isMemberOf  <microrelief> ;
  rdfs:label "Vertical interval"@en ;
  skos:definition "Give vertical distance, in metres, between base of depression or flat and horizontal line joining crests of mounds or hummocks."@en ;
  skos:inScheme <> ;
  skos:prefLabel "Vertical interval"@en ;
  skos:topConceptOf <> ;
.
 <other-microrelief-O>
  a skos:Collection ;
  a sosa:ObservableProperty ;
  dcterms:description "Other microrelief."@en ;
  dcterms:identifier "http://anzsoil.org/def/au/asls/land-surface/microrelief-O"^^xsd:anyURI ;
  ui:isMemberOf  <microrelief> ;
  rdfs:label "Other microrelief"@en ;
  skos:definition "Other microrelief."@en ;
  skos:inScheme <> ;
  skos:member  <microrelief-H> ;
  skos:member  <microrelief-I> ;
  skos:member  <microrelief-K> ;
  skos:member  <microrelief-P> ;
  skos:member  <microrelief-R> ;
  skos:member  <microrelief-S> ;
  skos:member  <microrelief-T> ;
  skos:member  <microrelief-U> ;
  skos:notation "O" ;
  skos:prefLabel "Other microrelief"@en ;
  skos:topConceptOf <> ;
.
 <rock-outcrop>
  a skos:Collection ;
  dcterms:description "This refers to any exposed area of rock that is inferred to be continuous with underlying bedrock."@en ;
  dcterms:identifier "http://anzsoil.org/def/au/asls/land-surface/rock-outcrop"^^xsd:anyURI ;
  ui:topMemberOf <> ;
  rdfs:label "Rock outcrop"@en ;
  skos:definition "This refers to any exposed area of rock that is inferred to be continuous with underlying bedrock."@en ;
  skos:member  <rock-outcrop-abundance> ;
  skos:member  <rock-outcrop-lithology> ;
  skos:prefLabel "Rock outcrop"@en ;
.
 <rock-outcrop-abundance>
  a skos:Collection ;
  a sosa:ObservableProperty ;
  dcterms:description "Abundance of rock outcrop."@en ;
  dcterms:identifier "http://anzsoil.org/def/au/asls/land-surface/rock-outcrop"^^xsd:anyURI ;
  ui:isMemberOf  <rock-outcrop> ;
  rdfs:label "Abundance of rock outcrop"@en ;
  skos:definition "Abundance of rock outcrop."@en ;
  skos:member  <rock-outcrop-abundance-0> ;
  skos:member  <rock-outcrop-abundance-1> ;
  skos:member  <rock-outcrop-abundance-2> ;
  skos:member  <rock-outcrop-abundance-3> ;
  skos:member  <rock-outcrop-abundance-4> ;
  skos:member  <rock-outcrop-abundance-5> ;
  skos:prefLabel "Abundance of rock outcrop"@en ;
.
 <rock-outcrop-abundance-0>
  a skos:Concept ;
  dcterms:description "no bedrock exposed."@en ;
  dcterms:identifier "http://anzsoil.org/def/au/asls/land-surface/rock-outcrop-abundance-0"^^xsd:anyURI ;
  ui:isMemberOf  <rock-outcrop-abundance> ;
  rdfs:label "No rock outcrop"@en ;
  skos:definition "no bedrock exposed."@en ;
  skos:inScheme <> ;
  skos:notation "0" ;
  skos:prefLabel "No rock outcrop"@en ;
  skos:topConceptOf <> ;
.
 <rock-outcrop-abundance-1>
  a skos:Concept ;
  dcterms:description "<2% bedrock exposed."@en ;
  dcterms:identifier "http://anzsoil.org/def/au/asls/land-surface/rock-outcrop-abundance-1"^^xsd:anyURI ;
  ui:isMemberOf  <rock-outcrop-abundance> ;
  rdfs:label "Very slightly rocky"@en ;
  skos:definition "<2% bedrock exposed."@en ;
  skos:inScheme <> ;
  skos:notation "1" ;
  skos:prefLabel "Very slightly rocky"@en ;
  skos:topConceptOf <> ;
.
 <rock-outcrop-abundance-2>
  a skos:Concept ;
  dcterms:description "2–10% bedrock exposed."@en ;
  dcterms:identifier "http://anzsoil.org/def/au/asls/land-surface/rock-outcrop-abundance-2"^^xsd:anyURI ;
  ui:isMemberOf  <rock-outcrop-abundance> ;
  rdfs:label "Slightly rocky"@en ;
  skos:definition "2–10% bedrock exposed."@en ;
  skos:inScheme <> ;
  skos:notation "2" ;
  skos:prefLabel "Slightly rocky"@en ;
  skos:topConceptOf <> ;
.
 <rock-outcrop-abundance-3>
  a skos:Concept ;
  dcterms:description "10–20% bedrock exposed."@en ;
  dcterms:identifier "http://anzsoil.org/def/au/asls/land-surface/rock-outcrop-abundance-3"^^xsd:anyURI ;
  ui:isMemberOf  <rock-outcrop-abundance> ;
  rdfs:label "Rocky"@en ;
  skos:definition "10–20% bedrock exposed."@en ;
  skos:inScheme <> ;
  skos:notation "3" ;
  skos:prefLabel "Rocky"@en ;
  skos:topConceptOf <> ;
.
 <rock-outcrop-abundance-4>
  a skos:Concept ;
  dcterms:description "20–50% bedrock exposed."@en ;
  dcterms:identifier "http://anzsoil.org/def/au/asls/land-surface/rock-outcrop-abundance-4"^^xsd:anyURI ;
  ui:isMemberOf  <rock-outcrop-abundance> ;
  rdfs:label "Very rocky"@en ;
  skos:definition "20–50% bedrock exposed."@en ;
  skos:inScheme <> ;
  skos:notation "4" ;
  skos:prefLabel "Very rocky"@en ;
  skos:topConceptOf <> ;
.
 <rock-outcrop-abundance-5>
  a skos:Concept ;
  dcterms:description ">50% bedrock exposed."@en ;
  dcterms:identifier "http://anzsoil.org/def/au/asls/land-surface/rock-outcrop-abundance-5"^^xsd:anyURI ;
  ui:isMemberOf  <rock-outcrop-abundance> ;
  rdfs:label "Rockland"@en ;
  skos:definition ">50% bedrock exposed."@en ;
  skos:inScheme <> ;
  skos:notation "5" ;
  skos:prefLabel "Rockland"@en ;
  skos:topConceptOf <> ;
.
 <rock-outcrop-lithology>
  a skos:Collection ;
  a sosa:ObservableProperty ;
  dcterms:description "Where the lithology of the rock outcrop is different from that of the substrate material, record it as for lithology of substrate material."@en ;
  dcterms:identifier "http://anzsoil.org/def/au/asls/land-surface/rock-outcrop-lithology"^^xsd:anyURI ;
  ui:isMemberOf  <rock-outcrop> ;
  rdfs:label "Lithology of rock outcrop"@en ;
  skos:definition "Where the lithology of the rock outcrop is different from that of the substrate material, record it as for lithology of substrate material. "@en ;
  skos:member  <../substrate/lithology-AC> ;
  skos:member  <../substrate/lithology-AD> ;
  skos:member  <../substrate/lithology-AF> ;
  skos:member  <../substrate/lithology-AG> ;
  skos:member  <../substrate/lithology-AH> ;
  skos:member  <../substrate/lithology-AM> ;
  skos:member  <../substrate/lithology-AN> ;
  skos:member  <../substrate/lithology-AP> ;
  skos:member  <../substrate/lithology-AR> ;
  skos:member  <../substrate/lithology-AS> ;
  skos:member  <../substrate/lithology-BA> ;
  skos:member  <../substrate/lithology-BB> ;
  skos:member  <../substrate/lithology-BR> ;
  skos:member  <../substrate/lithology-C> ;
  skos:member  <../substrate/lithology-CG> ;
  skos:member  <../substrate/lithology-CH> ;
  skos:member  <../substrate/lithology-CO> ;
  skos:member  <../substrate/lithology-CU> ;
  skos:member  <../substrate/lithology-DI> ;
  skos:member  <../substrate/lithology-DM> ;
  skos:member  <../substrate/lithology-DR> ;
  skos:member  <../substrate/lithology-FC> ;
  skos:member  <../substrate/lithology-GA> ;
  skos:member  <../substrate/lithology-GD> ;
  skos:member  <../substrate/lithology-GE> ;
  skos:member  <../substrate/lithology-GN> ;
  skos:member  <../substrate/lithology-GR> ;
  skos:member  <../substrate/lithology-GS> ;
  skos:member  <../substrate/lithology-GV> ;
  skos:member  <../substrate/lithology-GW> ;
  skos:member  <../substrate/lithology-GY> ;
  skos:member  <../substrate/lithology-HA> ;
  skos:member  <../substrate/lithology-HO> ;
  skos:member  <../substrate/lithology-IG> ;
  skos:member  <../substrate/lithology-JA> ;
  skos:member  <../substrate/lithology-KA> ;
  skos:member  <../substrate/lithology-KC> ;
  skos:member  <../substrate/lithology-KL> ;
  skos:member  <../substrate/lithology-KM> ;
  skos:member  <../substrate/lithology-KR> ;
  skos:member  <../substrate/lithology-KS> ;
  skos:member  <../substrate/lithology-LC> ;
  skos:member  <../substrate/lithology-LI> ;
  skos:member  <../substrate/lithology-M> ;
  skos:member  <../substrate/lithology-MB> ;
  skos:member  <../substrate/lithology-MD> ;
  skos:member  <../substrate/lithology-ME> ;
  skos:member  <../substrate/lithology-MG> ;
  skos:member  <../substrate/lithology-MI> ;
  skos:member  <../substrate/lithology-ML> ;
  skos:member  <../substrate/lithology-MS> ;
  skos:member  <../substrate/lithology-MU> ;
  skos:member  <../substrate/lithology-MY> ;
  skos:member  <../substrate/lithology-PC> ;
  skos:member  <../substrate/lithology-PE> ;
  skos:member  <../substrate/lithology-PG> ;
  skos:member  <../substrate/lithology-PH> ;
  skos:member  <../substrate/lithology-PL> ;
  skos:member  <../substrate/lithology-PO> ;
  skos:member  <../substrate/lithology-PY> ;
  skos:member  <../substrate/lithology-QP> ;
  skos:member  <../substrate/lithology-QS> ;
  skos:member  <../substrate/lithology-QU> ;
  skos:member  <../substrate/lithology-QZ> ;
  skos:member  <../substrate/lithology-R> ;
  skos:member  <../substrate/lithology-RB> ;
  skos:member  <../substrate/lithology-RH> ;
  skos:member  <../substrate/lithology-S> ;
  skos:member  <../substrate/lithology-SA> ;
  skos:member  <../substrate/lithology-SD> ;
  skos:member  <../substrate/lithology-SH> ;
  skos:member  <../substrate/lithology-SK> ;
  skos:member  <../substrate/lithology-SL> ;
  skos:member  <../substrate/lithology-SR> ;
  skos:member  <../substrate/lithology-ST> ;
  skos:member  <../substrate/lithology-SY> ;
  skos:member  <../substrate/lithology-TR> ;
  skos:member  <../substrate/lithology-TU> ;
  skos:member  <../substrate/lithology-UC> ;
  skos:member  <../substrate/lithology-VB> ;
  skos:member  <../substrate/lithology-VG> ;
  skos:member  <../substrate/lithology-Z> ;
  skos:member  <../substrate/lithology-ZS> ;
  skos:prefLabel "Lithology of rock outcrop"@en ;
.
 <runoff>
  a skos:Collection ;
  a sosa:ObservableProperty ;
  dcterms:description "Runoff is the relative rate at which water runs off the soil surface. It is largely determined by slope, surface cover and soil infiltration rate. "@en ;
  dcterms:identifier "http://anzsoil.org/def/au/asls/land-surface/runoff"^^xsd:anyURI ;
  ui:topMemberOf <> ;
  rdfs:label "Runoff"@en ;
  skos:definition "Runoff is the relative rate at which water runs off the soil surface. It is largely determined by slope, surface cover and soil infiltration rate. "@en ;
  skos:member  <runoff-0> ;
  skos:member  <runoff-1> ;
  skos:member  <runoff-2> ;
  skos:member  <runoff-3> ;
  skos:member  <runoff-4> ;
  skos:member  <runoff-5> ;
  skos:prefLabel "Runoff"@en ;
.
 <runoff-0>
  a skos:Concept ;
  dcterms:description "No runoff."@en ;
  dcterms:identifier "http://anzsoil.org/def/au/asls/land-surface/runoff-0"^^xsd:anyURI ;
  ui:isMemberOf  <runoff> ;
  rdfs:label "No runoff"@en ;
  skos:definition "No runoff."@en ;
  skos:inScheme <> ;
  skos:notation "0" ;
  skos:prefLabel "No runoff"@en ;
  skos:topConceptOf <> ;
.
 <runoff-1>
  a skos:Concept ;
  dcterms:description "free water on surface for long periods, or water enters soil immediately. Soils usually either level to nearly level or loose and porous."@en ;
  dcterms:identifier "http://anzsoil.org/def/au/asls/land-surface/runoff-1"^^xsd:anyURI ;
  ui:isMemberOf  <runoff> ;
  rdfs:label "Very slow"@en ;
  skos:definition "free water on surface for long periods, or water enters soil immediately. Soils usually either level to nearly level or loose and porous."@en ;
  skos:inScheme <> ;
  skos:notation "1" ;
  skos:prefLabel "Very slow"@en ;
  skos:topConceptOf <> ;
.
 <runoff-2>
  a skos:Concept ;
  dcterms:description "free water on surface for significant periods, or water enters soil relatively rapidly. Soils usually either nearly level to gently sloping or relatively porous."@en ;
  dcterms:identifier "http://anzsoil.org/def/au/asls/land-surface/runoff-2"^^xsd:anyURI ;
  ui:isMemberOf  <runoff> ;
  rdfs:label "Slow"@en ;
  skos:definition "free water on surface for significant periods, or water enters soil relatively rapidly. Soils usually either nearly level to gently sloping or relatively porous."@en ;
  skos:inScheme <> ;
  skos:notation "2" ;
  skos:prefLabel "Slow"@en ;
  skos:topConceptOf <> ;
.
 <runoff-3>
  a skos:Concept ;
  dcterms:description "free water on surface for short periods only; moderate proportion of water enters soil."@en ;
  dcterms:identifier "http://anzsoil.org/def/au/asls/land-surface/runoff-3"^^xsd:anyURI ;
  ui:isMemberOf  <runoff> ;
  rdfs:label "Moderately rapid"@en ;
  skos:definition "free water on surface for short periods only; moderate proportion of water enters soil."@en ;
  skos:inScheme <> ;
  skos:notation "3" ;
  skos:prefLabel "Moderately rapid"@en ;
  skos:topConceptOf <> ;
.
 <runoff-4>
  a skos:Concept ;
  dcterms:description "large proportion of water runs off; small proportion enters soil. Water runs off nearly as fast as it is added. Soils usually have moderate to steep slopes and low infiltration rates."@en ;
  dcterms:identifier "http://anzsoil.org/def/au/asls/land-surface/runoff-4"^^xsd:anyURI ;
  ui:isMemberOf  <runoff> ;
  rdfs:label "Rapid"@en ;
  skos:definition "large proportion of water runs off; small proportion enters soil. Water runs off nearly as fast as it is added. Soils usually have moderate to steep slopes and low infiltration rates."@en ;
  skos:inScheme <> ;
  skos:notation "4" ;
  skos:prefLabel "Rapid"@en ;
  skos:topConceptOf <> ;
.
 <runoff-5>
  a skos:Concept ;
  dcterms:description "very large proportion of water runs off; very small proportion enters soil. Water runs off as fast as it is added. Soils usually have steep to very steep slopes and low infiltration rates."@en ;
  dcterms:identifier "http://anzsoil.org/def/au/asls/land-surface/runoff-5"^^xsd:anyURI ;
  ui:isMemberOf  <runoff> ;
  rdfs:label "Very rapid"@en ;
  skos:definition "very large proportion of water runs off; very small proportion enters soil. Water runs off as fast as it is added. Soils usually have steep to very steep slopes and low infiltration rates."@en ;
  skos:inScheme <> ;
  skos:notation "5" ;
  skos:prefLabel "Very rapid"@en ;
  skos:topConceptOf <> ;
.
 <water-erosion>
  a skos:Collection ;
  dcterms:description """Give type and presence/absence or extent of accelerated erosion.
For sheet, rill and gully erosion there is no consensus in Australia on a quantitative or precise definition of what constitutes minor, moderate and severe erosion. This derives partly from the difficulty of measuring actual soil loss at a site. It also derives partly from the wide range of soils, climates and land uses, variations in any or all of which may alter the concept of minor, moderate or severe erosion.
The observer wishing to record the severity of erosion may record it as minor, moderate or severe, basing the assessment on local knowledge and guided by indicators that may be present as described below (after Morse et al. 1987). Note the actual depth of soil loss where this can be reliably assessed."""@en ;
  dcterms:identifier "http://anzsoil.org/def/au/asls/land-surface/water-erosion"^^xsd:anyURI ;
  ui:isMemberOf  <erosion> ;
  rdfs:label "Water erosion"@en ;
  skos:definition """Give type and presence/absence or extent of accelerated erosion.
For sheet, rill and gully erosion there is no consensus in Australia on a quantitative or precise definition of what constitutes minor, moderate and severe erosion. This derives partly from the difficulty of measuring actual soil loss at a site. It also derives partly from the wide range of soils, climates and land uses, variations in any or all of which may alter the concept of minor, moderate or severe erosion.
The observer wishing to record the severity of erosion may record it as minor, moderate or severe, basing the assessment on local knowledge and guided by indicators that may be present as described below (after Morse et al. 1987). Note the actual depth of soil loss where this can be reliably assessed."""@en ;
  skos:member  <erosion-B> ;
  skos:member  <erosion-G> ;
  skos:member  <erosion-R> ;
  skos:member  <erosion-S> ;
  skos:member  <erosion-T> ;
  skos:member  <erosion-V> ;
  skos:prefLabel "Water erosion"@en ;
.
